@prefix owl: <http://www.w3.org/2002/07/owl#> .
@prefix rdf: <http://www.w3.org/1999/02/22-rdf-syntax-ns#> .
@prefix rdfs: <http://www.w3.org/2000/01/rdf-schema#> .
@prefix sbvr: <https://www.omg.org/spec/SBVR/20190601#> .
@prefix skos: <http://www.w3.org/2004/02/skos/core#> .
@prefix xsd: <http://www.w3.org/2001/XMLSchema#> .

sbvr:adoptingAuthority a rdf:Property ;
    rdfs:comment "This is the adoptingAuthority property or class within the SBVR ontology." ;
    rdfs:domain sbvr:AdoptingAuthorityAdoptsElementOfGuidanceFromOwningAuthorityCitingReference ;
    rdfs:range xsd:anyType .

sbvr:antecedent a rdf:Property ;
    rdfs:comment "This is the antecedent property or class within the SBVR ontology." ;
    rdfs:domain sbvr:Implication,
        sbvr:Implicationhasantecedent ;
    rdfs:range xsd:anyType .

sbvr:binaryLogicalOperation a rdf:Property ;
    rdfs:comment "This is the binaryLogicalOperation property or class within the SBVR ontology." ;
    rdfs:domain sbvr:BinaryLogicalOperationHasLogicalOperand1,
        sbvr:BinaryLogicalOperationHasLogicalOperand2 .

sbvr:bindableTarget a rdf:Property ;
    rdfs:comment "This is the bindableTarget property or class within the SBVR ontology." ;
    rdfs:domain sbvr:Instantiationformulationbindstobindabletarget,
        sbvr:Objectificationbindstobindabletarget,
        sbvr:Projectingformulationbindstobindabletarget,
        sbvr:Propositionnominalizationbindstobindabletarget,
        sbvr:Rolebindingbindstobindabletarget .

sbvr:bodyOfSharedMeanings1 a rdf:Property ;
    rdfs:comment "This is the bodyOfSharedMeanings1 property or class within the SBVR ontology." ;
    rdfs:domain sbvr:Bodyofsharedmeanings1containsbodyofsharedmeanings2 .

sbvr:bodyOfSharedMeanings2 a rdf:Property ;
    rdfs:comment "This is the bodyOfSharedMeanings2 property or class within the SBVR ontology." ;
    rdfs:domain sbvr:Bodyofsharedmeanings1containsbodyofsharedmeanings2 .

sbvr:cardinality a rdf:Property ;
    rdfs:comment "This is the cardinality property or class within the SBVR ontology." ;
    rdfs:domain sbvr:Bodyofsharedmeanings,
        sbvr:Businessvocabulary,
        sbvr:ExactlyNQuantification,
        sbvr:ExactlyNQuantificationHasCardinality,
        sbvr:ExactlyOneQuantification,
        sbvr:RuleSet,
        sbvr:Sethascardinality,
        sbvr:Speechcommunityrepresentationset,
        sbvr:Vocabulary ;
    rdfs:range xsd:anyType .

sbvr:category a rdf:Property ;
    rdfs:comment "This is the category property or class within the SBVR ontology." ;
    rdfs:domain sbvr:Association,
        sbvr:Binaryverbconcept,
        sbvr:Categorizationschemecontainscategory,
        sbvr:Categorizationtype,
        sbvr:Characteristic,
        sbvr:Characteristictype,
        sbvr:Conceptofthingascomposite,
        sbvr:ConceptOfThingAsContinuant,
        sbvr:ConceptOfThingAsDeveloped,
        sbvr:Conceptofthingasoccurrent,
        sbvr:Conceptofthingasprimitive,
        sbvr:Conceptofthingasunitary,
        sbvr:Conceptofthingexistingdependently,
        sbvr:Conceptofthingexistingindependently,
        sbvr:Concepttype,
        sbvr:Contextualizedconcept,
        sbvr:Derivableconcept,
        sbvr:Facet,
        sbvr:Fundamentalconcept,
        sbvr:GeneralConcept,
        sbvr:GeneralVerbConcept,
        sbvr:IndividualNounConcept,
        sbvr:Integer,
        sbvr:LogicalFormulationKind,
        sbvr:NonNegativeInteger,
        sbvr:NounConcept,
        sbvr:Number,
        sbvr:PartitiveVerbConcept,
        sbvr:PositiveInteger,
        sbvr:PropertyAssociation,
        sbvr:Quantity,
        sbvr:Role,
        sbvr:SituationalRole,
        sbvr:Unitaryverbconcept,
        sbvr:VerbConcept,
        sbvr:VerbConceptRole ;
    rdfs:range xsd:anyType .

sbvr:closeMatch a rdf:Property ;
    rdfs:label "close match" ;
    rdfs:comment "Links an sbvr:term to a skos:Concept that has the closest meaning. When used to connect terms in a similarity search, means the term has at least a 80% match",
        "This is the closeMatch property or class within the SBVR ontology." ;
    rdfs:domain sbvr:Term ;
    rdfs:range skos:Concept ;
    rdfs:subPropertyOf skos:closeMatch .

sbvr:closedSemanticFormulation a rdf:Property ;
    rdfs:comment "This is the closedSemanticFormulation property or class within the SBVR ontology." ;
    rdfs:domain sbvr:Closedsemanticformulationformulatesmeaning .

sbvr:community a rdf:Property ;
    rdfs:comment "This is the community property or class within the SBVR ontology." ;
    rdfs:domain sbvr:Communityhassubcommunity,
        sbvr:CommunityHasUri .

sbvr:concept a rdf:Property ;
    rdfs:comment "Unit of knowledge created by a unique combination of characteristics." ;
    rdfs:domain sbvr:BodyOfSharedConceptsIncludesConcept,
        sbvr:ConceptHasDefinition,
        sbvr:ConceptHasDesignation,
        sbvr:ConceptHasExtension,
        sbvr:ConceptHasFacet,
        sbvr:ConceptHasImpliedCharacteristic,
        sbvr:ConceptHasInstance,
        sbvr:ConceptHasNecessaryCharacteristic,
        sbvr:ConceptIncorporatesCharacteristic,
        sbvr:Instantiationformulationconsidersconcept,
        sbvr:ReferenceSchemeisforconcept,
        sbvr:Semanticcommunitysharesunderstandingofconcept,
        sbvr:Variablerangesoverconcept .

sbvr:concept1 a rdf:Property ;
    rdfs:comment "This is the concept1 property or class within the SBVR ontology." ;
    rdfs:domain sbvr:Concept1iscoextensivewithconcept2,
        sbvr:Concept1specializesconcept2 .

sbvr:concept2 a rdf:Property ;
    rdfs:comment "This is the concept2 property or class within the SBVR ontology." ;
    rdfs:domain sbvr:Concept1iscoextensivewithconcept2,
        sbvr:Concept1specializesconcept2 .

sbvr:consequent a rdf:Property ;
    rdfs:comment "This is the consequent property or class within the SBVR ontology." ;
    rdfs:domain sbvr:Implication,
        sbvr:Implicationhasconsequent,
        sbvr:WhetherOrNotFormulation,
        sbvr:WhetherOrNotFormulationHasConsequent ;
    rdfs:range xsd:anyType .

sbvr:constrainingFormulation a rdf:Property ;
    rdfs:comment "This is the constrainingFormulation property or class within the SBVR ontology." ;
    rdfs:domain sbvr:Bagprojection,
        sbvr:Closedprojection,
        sbvr:Projection,
        sbvr:SetProjection ;
    rdfs:range xsd:anyType .

sbvr:delimitingCharacteristic a rdf:Property ;
    rdfs:comment "This is the delimitingCharacteristic property or class within the SBVR ontology." ;
    rdfs:domain sbvr:IntensionalDefinitionusesdelimitingcharacteristic .

sbvr:designationContext a rdf:Property ;
    rdfs:comment "This is the designationContext property or class within the SBVR ontology." ;
    rdfs:domain sbvr:Representationisindesignationcontext,
        sbvr:VocabularyNamespaceIsSpecificToDesignationContext .

sbvr:element a rdf:Property ;
    rdfs:comment "This is the element property or class within the SBVR ontology." ;
    rdfs:domain sbvr:Bodyofsharedmeanings,
        sbvr:Businessvocabulary,
        sbvr:RuleSet,
        sbvr:Speechcommunityrepresentationset,
        sbvr:Vocabulary ;
    rdfs:range xsd:anyType .

sbvr:essentialCharacteristic a rdf:Property ;
    rdfs:comment "This is the essentialCharacteristic property or class within the SBVR ontology." ;
    rdfs:domain sbvr:Association,
        sbvr:Binaryverbconcept,
        sbvr:Categorizationtype,
        sbvr:Characteristic,
        sbvr:Characteristictype,
        sbvr:Conceptofthingascomposite,
        sbvr:ConceptOfThingAsContinuant,
        sbvr:ConceptOfThingAsDeveloped,
        sbvr:Conceptofthingasoccurrent,
        sbvr:Conceptofthingasprimitive,
        sbvr:Conceptofthingasunitary,
        sbvr:Conceptofthingexistingdependently,
        sbvr:Conceptofthingexistingindependently,
        sbvr:Concepttype,
        sbvr:Contextualizedconcept,
        sbvr:Derivableconcept,
        sbvr:Facet,
        sbvr:Fundamentalconcept,
        sbvr:GeneralConcept,
        sbvr:GeneralVerbConcept,
        sbvr:IndividualNounConcept,
        sbvr:Integer,
        sbvr:LogicalFormulationKind,
        sbvr:NonNegativeInteger,
        sbvr:NounConcept,
        sbvr:Number,
        sbvr:PartitiveVerbConcept,
        sbvr:PositiveInteger,
        sbvr:PropertyAssociation,
        sbvr:Quantity,
        sbvr:Role,
        sbvr:SituationalRole,
        sbvr:Unitaryverbconcept,
        sbvr:VerbConcept,
        sbvr:VerbConceptRole ;
    rdfs:range xsd:anyType .

sbvr:exactMatch a rdf:Property ;
    rdfs:label "exact match" ;
    rdfs:comment "Links an sbvr:term to a skos:Concept that has the same meaning. When used to connect terms in a similarity search, means the term has at least a 99% match",
        "This is the exactMatch property or class within the SBVR ontology." ;
    rdfs:domain sbvr:Term ;
    rdfs:range skos:Concept ;
    rdfs:subPropertyOf skos:exactMatch .

sbvr:expression a rdf:Property ;
    rdfs:comment "Something that expresses or communicates, but considered independently of its interpretation. Example: the sequence of characters 'car'",
        "This is the expression property or class within the SBVR ontology." ;
    rdfs:domain sbvr:AdoptedDefinition,
        sbvr:Advicestatement,
        sbvr:BehavioralBusinessRulestatement,
        sbvr:Businesspolicystatement,
        sbvr:Communicationcontent,
        sbvr:Contingencystatement,
        sbvr:Definitedescription,
        sbvr:Definition,
        sbvr:DefinitionalRuleStatement,
        sbvr:Description,
        sbvr:Descriptiveexample,
        sbvr:Designation,
        sbvr:Expressionisunambiguoustospeechcommunity,
        sbvr:Expressionrepresentsmeaning,
        sbvr:Extensionaldefinition,
        sbvr:FormalRepresentation,
        sbvr:GuidanceStatement,
        sbvr:Icon,
        sbvr:Impossibilitystatement,
        sbvr:InFormalRepresentation,
        sbvr:IntensionalDefinition,
        sbvr:Name,
        sbvr:NecessityStatement,
        sbvr:NonNecessityStatement,
        sbvr:NonObligationStatement,
        sbvr:Nonverbaldesignation,
        sbvr:Note,
        sbvr:Nounform,
        sbvr:ObligationStatement,
        sbvr:Optionalitystatement,
        sbvr:Owneddefinition,
        sbvr:Permissionstatement,
        sbvr:Placeholder,
        sbvr:Possibilitystatement,
        sbvr:Preferreddesignation,
        sbvr:Prohibiteddesignation,
        sbvr:Prohibitionstatement,
        sbvr:Reference,
        sbvr:Representation,
        sbvr:RepresentationHasExpression,
        sbvr:Restrictedpermissionstatement,
        sbvr:Restrictedpossibilitystatement,
        sbvr:Rulestatement,
        sbvr:SententialForm,
        sbvr:Statement,
        sbvr:StatementOfAdviceOfPermission,
        sbvr:StatementofAdviceOfPossibility,
        sbvr:Term,
        sbvr:VerbConceptRoledesignation,
        sbvr:VerbConceptwording,
        sbvr:Verbsymbol ;
    rdfs:range xsd:anyType .

sbvr:extension a rdf:Property ;
    rdfs:comment "This is the extension property or class within the SBVR ontology." ;
    rdfs:domain sbvr:Association,
        sbvr:Binaryverbconcept,
        sbvr:Categorizationtype,
        sbvr:Characteristic,
        sbvr:Characteristictype,
        sbvr:ConceptHasExtension,
        sbvr:Conceptofthingascomposite,
        sbvr:ConceptOfThingAsContinuant,
        sbvr:ConceptOfThingAsDeveloped,
        sbvr:Conceptofthingasoccurrent,
        sbvr:Conceptofthingasprimitive,
        sbvr:Conceptofthingasunitary,
        sbvr:Conceptofthingexistingdependently,
        sbvr:Conceptofthingexistingindependently,
        sbvr:Concepttype,
        sbvr:Contextualizedconcept,
        sbvr:Derivableconcept,
        sbvr:Facet,
        sbvr:Fundamentalconcept,
        sbvr:GeneralConcept,
        sbvr:GeneralVerbConcept,
        sbvr:IndividualNounConcept,
        sbvr:Integer,
        sbvr:LogicalFormulationKind,
        sbvr:NonNegativeInteger,
        sbvr:NounConcept,
        sbvr:Number,
        sbvr:PartitiveVerbConcept,
        sbvr:PositiveInteger,
        sbvr:PropertyAssociation,
        sbvr:Quantity,
        sbvr:Role,
        sbvr:SituationalRole,
        sbvr:Unitaryverbconcept,
        sbvr:VerbConcept,
        sbvr:VerbConceptRole ;
    rdfs:range xsd:anyType .

sbvr:extensionallyUsedRole a rdf:Property ;
    rdfs:comment "This is the extensionallyUsedRole property or class within the SBVR ontology." ;
    rdfs:domain sbvr:ReferenceScheme ;
    rdfs:range xsd:anyType .

sbvr:identifyingCharacteristic a rdf:Property ;
    rdfs:comment "This is the identifyingCharacteristic property or class within the SBVR ontology." ;
    rdfs:domain sbvr:ReferenceScheme ;
    rdfs:range xsd:anyType .

sbvr:impliedCharacteristic a rdf:Property ;
    rdfs:comment "This is the impliedCharacteristic property or class within the SBVR ontology." ;
    rdfs:domain sbvr:Association,
        sbvr:Binaryverbconcept,
        sbvr:Categorizationtype,
        sbvr:Characteristic,
        sbvr:Characteristictype,
        sbvr:ConceptHasImpliedCharacteristic,
        sbvr:Conceptofthingascomposite,
        sbvr:ConceptOfThingAsContinuant,
        sbvr:ConceptOfThingAsDeveloped,
        sbvr:Conceptofthingasoccurrent,
        sbvr:Conceptofthingasprimitive,
        sbvr:Conceptofthingasunitary,
        sbvr:Conceptofthingexistingdependently,
        sbvr:Conceptofthingexistingindependently,
        sbvr:Concepttype,
        sbvr:Contextualizedconcept,
        sbvr:Derivableconcept,
        sbvr:Facet,
        sbvr:Fundamentalconcept,
        sbvr:GeneralConcept,
        sbvr:GeneralVerbConcept,
        sbvr:IndividualNounConcept,
        sbvr:Integer,
        sbvr:LogicalFormulationKind,
        sbvr:NonNegativeInteger,
        sbvr:NounConcept,
        sbvr:Number,
        sbvr:PartitiveVerbConcept,
        sbvr:PositiveInteger,
        sbvr:PropertyAssociation,
        sbvr:Quantity,
        sbvr:Role,
        sbvr:SituationalRole,
        sbvr:Unitaryverbconcept,
        sbvr:VerbConcept,
        sbvr:VerbConceptRole ;
    rdfs:range xsd:anyType .

sbvr:inconsequent a rdf:Property ;
    rdfs:comment "This is the inconsequent property or class within the SBVR ontology." ;
    rdfs:domain sbvr:WhetherOrNotFormulation,
        sbvr:WhetherOrNotFormulationHasInconsequent ;
    rdfs:range xsd:anyType .

sbvr:informationSource a rdf:Property ;
    rdfs:comment "This is the informationSource property or class within the SBVR ontology." ;
    rdfs:domain sbvr:ReferencePointsToInformationSource .

sbvr:instance a rdf:Property ;
    rdfs:comment "This is the instance property or class within the SBVR ontology." ;
    rdfs:domain sbvr:Association,
        sbvr:Binaryverbconcept,
        sbvr:Categorizationtype,
        sbvr:Characteristic,
        sbvr:Characteristictype,
        sbvr:ConceptHasInstance,
        sbvr:Conceptofthingascomposite,
        sbvr:ConceptOfThingAsContinuant,
        sbvr:ConceptOfThingAsDeveloped,
        sbvr:Conceptofthingasoccurrent,
        sbvr:Conceptofthingasprimitive,
        sbvr:Conceptofthingasunitary,
        sbvr:Conceptofthingexistingdependently,
        sbvr:Conceptofthingexistingindependently,
        sbvr:Concepttype,
        sbvr:Contextualizedconcept,
        sbvr:Derivableconcept,
        sbvr:Facet,
        sbvr:Fundamentalconcept,
        sbvr:GeneralConcept,
        sbvr:GeneralVerbConcept,
        sbvr:IndividualNounConcept,
        sbvr:Integer,
        sbvr:LogicalFormulationKind,
        sbvr:NonNegativeInteger,
        sbvr:NounConcept,
        sbvr:Number,
        sbvr:PartitiveVerbConcept,
        sbvr:PositiveInteger,
        sbvr:PropertyAssociation,
        sbvr:Quantity,
        sbvr:Role,
        sbvr:SituationalRole,
        sbvr:Unitaryverbconcept,
        sbvr:VerbConcept,
        sbvr:VerbConceptRole ;
    rdfs:range xsd:anyType .

sbvr:isDirectlyEnforceable a rdf:Property ;
    rdfs:comment "This is the isDirectlyEnforceable property or class within the SBVR ontology." ;
    rdfs:domain sbvr:BehavioralBusinessRule,
        sbvr:Businesspolicy,
        sbvr:Elementofgovernance ;
    rdfs:range xsd:boolean .

sbvr:isImplicitlyUnderstood a rdf:Property ;
    rdfs:comment "Generally understood by its owning community without an explicit definition for the concept it designates",
        "This is the isImplicitlyUnderstood property or class within the SBVR ontology." ;
    rdfs:domain sbvr:Designation,
        sbvr:Icon,
        sbvr:Name,
        sbvr:Nonverbaldesignation,
        sbvr:Placeholder,
        sbvr:Preferreddesignation,
        sbvr:Prohibiteddesignation,
        sbvr:Term,
        sbvr:VerbConceptRoledesignation,
        sbvr:Verbsymbol ;
    rdfs:range xsd:boolean .

sbvr:isPracticable a rdf:Property ;
    rdfs:comment "This is the isPracticable property or class within the SBVR ontology." ;
    rdfs:domain sbvr:Advice,
        sbvr:AdviceOfContingency,
        sbvr:AdviceOfOptionality,
        sbvr:AdviceOfPermission,
        sbvr:AdviceOfPossibility,
        sbvr:BehavioralBusinessRule,
        sbvr:Businesspolicy,
        sbvr:Businessrule,
        sbvr:Elementofgovernance,
        sbvr:Elementofguidance ;
    rdfs:range xsd:boolean .

sbvr:isUnitary a rdf:Property ;
    rdfs:comment "This is the isUnitary property or class within the SBVR ontology." ;
    rdfs:domain sbvr:Auxiliaryvariable,
        sbvr:Variable ;
    rdfs:range xsd:boolean .

sbvr:isViolated a rdf:Property ;
    rdfs:comment "This is the isViolated property or class within the SBVR ontology." ;
    rdfs:domain sbvr:BehavioralBusinessRule ;
    rdfs:range xsd:boolean .

sbvr:logicalFormulation a rdf:Property ;
    rdfs:comment "This is the logicalFormulation property or class within the SBVR ontology." ;
    rdfs:domain sbvr:Logicalformulationconstrainsprojection,
        sbvr:Logicalformulationrestrictsvariable,
        sbvr:Modalformulationembedslogicalformulation,
        sbvr:Objectificationconsiderslogicalformulation,
        sbvr:Propositionnominalizationconsiderslogicalformulation,
        sbvr:Quantificationscopesoverlogicalformulation .

sbvr:logicalOperand a rdf:Property ;
    rdfs:comment "This is the logicalOperand property or class within the SBVR ontology." ;
    rdfs:domain sbvr:Conjunction,
        sbvr:Disjunction,
        sbvr:Equivalence,
        sbvr:Exclusivedisjunction,
        sbvr:Implication,
        sbvr:Logicalnegation,
        sbvr:Logicaloperationhaslogicaloperand,
        sbvr:Nandformulation,
        sbvr:Norformulation,
        sbvr:WhetherOrNotFormulation ;
    rdfs:range xsd:anyType .

sbvr:logicalOperand1 a rdf:Property ;
    rdfs:comment "This is the logicalOperand1 property or class within the SBVR ontology." ;
    rdfs:domain sbvr:BinaryLogicalOperationHasLogicalOperand1,
        sbvr:Conjunction,
        sbvr:Disjunction,
        sbvr:Equivalence,
        sbvr:Exclusivedisjunction,
        sbvr:Implication,
        sbvr:Nandformulation,
        sbvr:Norformulation,
        sbvr:WhetherOrNotFormulation ;
    rdfs:range xsd:anyType .

sbvr:logicalOperand2 a rdf:Property ;
    rdfs:comment "This is the logicalOperand2 property or class within the SBVR ontology." ;
    rdfs:domain sbvr:BinaryLogicalOperationHasLogicalOperand2,
        sbvr:Conjunction,
        sbvr:Disjunction,
        sbvr:Equivalence,
        sbvr:Exclusivedisjunction,
        sbvr:Implication,
        sbvr:Nandformulation,
        sbvr:Norformulation,
        sbvr:WhetherOrNotFormulation ;
    rdfs:range xsd:anyType .

sbvr:logicalOperation a rdf:Property ;
    rdfs:comment "This is the logicalOperation property or class within the SBVR ontology." ;
    rdfs:domain sbvr:Logicaloperationhaslogicaloperand .

sbvr:maximumCardinality a rdf:Property ;
    rdfs:comment "This is the maximumCardinality property or class within the SBVR ontology." ;
    rdfs:domain sbvr:AtMostNQuantification,
        sbvr:AtMostNQuantificationHasMaximumCardinality,
        sbvr:AtMostOneQuantification,
        sbvr:NumericrangeQuantification,
        sbvr:NumericrangeQuantificationhasmaximumcardinality ;
    rdfs:range xsd:anyType .

sbvr:meaning a rdf:Property ;
    rdfs:comment "What is meant by a word, sign, statement (natural language meaning), or description; what someone intends to express or what someone understands" ;
    rdfs:domain sbvr:AdoptedDefinition,
        sbvr:Advicestatement,
        sbvr:BehavioralBusinessRulestatement,
        sbvr:Businesspolicystatement,
        sbvr:Closedsemanticformulationformulatesmeaning,
        sbvr:Communicationcontent,
        sbvr:Contingencystatement,
        sbvr:Definitedescription,
        sbvr:Definition,
        sbvr:DefinitionalRuleStatement,
        sbvr:Description,
        sbvr:DescriptionPortraysMeaning,
        sbvr:Descriptiveexample,
        sbvr:DescriptiveExampleIllustratesMeaning,
        sbvr:Designation,
        sbvr:Expressionrepresentsmeaning,
        sbvr:Extensionaldefinition,
        sbvr:FormalRepresentation,
        sbvr:GuidanceStatement,
        sbvr:Icon,
        sbvr:Impossibilitystatement,
        sbvr:InFormalRepresentation,
        sbvr:IntensionalDefinition,
        sbvr:Name,
        sbvr:NecessityStatement,
        sbvr:NonNecessityStatement,
        sbvr:NonObligationStatement,
        sbvr:Nonverbaldesignation,
        sbvr:Note,
        sbvr:NoteCommentsOnMeaning,
        sbvr:Nounform,
        sbvr:ObligationStatement,
        sbvr:Optionalitystatement,
        sbvr:Owneddefinition,
        sbvr:Permissionstatement,
        sbvr:Placeholder,
        sbvr:Possibilitystatement,
        sbvr:Preferreddesignation,
        sbvr:Prohibiteddesignation,
        sbvr:Prohibitionstatement,
        sbvr:Reference,
        sbvr:ReferenceSupportsMeaning,
        sbvr:Representation,
        sbvr:Representationrepresentsmeaning,
        sbvr:Restrictedpermissionstatement,
        sbvr:Restrictedpossibilitystatement,
        sbvr:Rulestatement,
        sbvr:SententialForm,
        sbvr:Statement,
        sbvr:StatementOfAdviceOfPermission,
        sbvr:StatementofAdviceOfPossibility,
        sbvr:Term,
        sbvr:VerbConceptRoledesignation,
        sbvr:VerbConceptwording,
        sbvr:Verbsymbol ;
    rdfs:range xsd:anyType .

sbvr:minimumCardinality a rdf:Property ;
    rdfs:comment "This is the minimumCardinality property or class within the SBVR ontology." ;
    rdfs:domain sbvr:AtLeastNQuantification,
        sbvr:AtLeastNQuantificationHasMinimumCardinality,
        sbvr:ExistentialQuantification,
        sbvr:NumericrangeQuantification,
        sbvr:NumericrangeQuantificationhasminimumcardinality ;
    rdfs:range xsd:anyType .

sbvr:modalFormulation a rdf:Property ;
    rdfs:comment "This is the modalFormulation property or class within the SBVR ontology." ;
    rdfs:domain sbvr:Modalformulationembedslogicalformulation .

sbvr:moreGeneralConcept a rdf:Property ;
    rdfs:comment "This is the moreGeneralConcept property or class within the SBVR ontology." ;
    rdfs:domain sbvr:Association,
        sbvr:Binaryverbconcept,
        sbvr:Categorizationtype,
        sbvr:Characteristic,
        sbvr:Characteristictype,
        sbvr:Conceptofthingascomposite,
        sbvr:ConceptOfThingAsContinuant,
        sbvr:ConceptOfThingAsDeveloped,
        sbvr:Conceptofthingasoccurrent,
        sbvr:Conceptofthingasprimitive,
        sbvr:Conceptofthingasunitary,
        sbvr:Conceptofthingexistingdependently,
        sbvr:Conceptofthingexistingindependently,
        sbvr:Concepttype,
        sbvr:Contextualizedconcept,
        sbvr:Derivableconcept,
        sbvr:Facet,
        sbvr:Fundamentalconcept,
        sbvr:GeneralConcept,
        sbvr:GeneralVerbConcept,
        sbvr:IndividualNounConcept,
        sbvr:Integer,
        sbvr:LogicalFormulationKind,
        sbvr:NonNegativeInteger,
        sbvr:NounConcept,
        sbvr:Number,
        sbvr:PartitiveVerbConcept,
        sbvr:PositiveInteger,
        sbvr:PropertyAssociation,
        sbvr:Quantity,
        sbvr:Role,
        sbvr:SituationalRole,
        sbvr:Unitaryverbconcept,
        sbvr:VerbConcept,
        sbvr:VerbConceptRole ;
    rdfs:range xsd:anyType .

sbvr:namespace1 a rdf:Property ;
    rdfs:comment "This is the namespace1 property or class within the SBVR ontology." ;
    rdfs:domain sbvr:Namespace1incorporatesnamespace2 .

sbvr:namespace2 a rdf:Property ;
    rdfs:comment "This is the namespace2 property or class within the SBVR ontology." ;
    rdfs:domain sbvr:Namespace1incorporatesnamespace2 .

sbvr:necessaryCharacteristic a rdf:Property ;
    rdfs:comment "This is the necessaryCharacteristic property or class within the SBVR ontology." ;
    rdfs:domain sbvr:Association,
        sbvr:Binaryverbconcept,
        sbvr:Categorizationtype,
        sbvr:Characteristic,
        sbvr:Characteristictype,
        sbvr:ConceptHasNecessaryCharacteristic,
        sbvr:Conceptofthingascomposite,
        sbvr:ConceptOfThingAsContinuant,
        sbvr:ConceptOfThingAsDeveloped,
        sbvr:Conceptofthingasoccurrent,
        sbvr:Conceptofthingasprimitive,
        sbvr:Conceptofthingasunitary,
        sbvr:Conceptofthingexistingdependently,
        sbvr:Conceptofthingexistingindependently,
        sbvr:Concepttype,
        sbvr:Contextualizedconcept,
        sbvr:Derivableconcept,
        sbvr:Facet,
        sbvr:Fundamentalconcept,
        sbvr:GeneralConcept,
        sbvr:GeneralVerbConcept,
        sbvr:IndividualNounConcept,
        sbvr:Integer,
        sbvr:LogicalFormulationKind,
        sbvr:NonNegativeInteger,
        sbvr:NounConcept,
        sbvr:Number,
        sbvr:PartitiveVerbConcept,
        sbvr:PositiveInteger,
        sbvr:PropertyAssociation,
        sbvr:Quantity,
        sbvr:Role,
        sbvr:SituationalRole,
        sbvr:Unitaryverbconcept,
        sbvr:VerbConcept,
        sbvr:VerbConceptRole ;
    rdfs:range xsd:anyType .

sbvr:objectifiedVerbConcept a rdf:Property ;
    rdfs:comment "This is the objectifiedVerbConcept property or class within the SBVR ontology." ;
    rdfs:domain sbvr:Categorizationtype,
        sbvr:Characteristictype,
        sbvr:Concepttype,
        sbvr:Fundamentalconcept,
        sbvr:GeneralConcept,
        sbvr:LogicalFormulationKind,
        sbvr:SituationalRole ;
    rdfs:range xsd:anyType .

sbvr:owningAuthority a rdf:Property ;
    rdfs:comment "This is the owningAuthority property or class within the SBVR ontology." ;
    rdfs:domain sbvr:AdoptingAuthorityAdoptsElementOfGuidanceFromOwningAuthorityCitingReference ;
    rdfs:range xsd:anyType .

sbvr:projectingFormulation a rdf:Property ;
    rdfs:comment "This is the projectingFormulation property or class within the SBVR ontology." ;
    rdfs:domain sbvr:Projectingformulationbindstobindabletarget,
        sbvr:Projectingformulationhasprojection .

sbvr:projectionPosition a rdf:Property ;
    rdfs:comment "This is the projectionPosition property or class within the SBVR ontology." ;
    rdfs:domain sbvr:Auxiliaryvariable,
        sbvr:Variable,
        sbvr:Variablehasprojectionposition ;
    rdfs:range xsd:anyType .

sbvr:projectionVariable a rdf:Property ;
    rdfs:comment "This is the projectionVariable property or class within the SBVR ontology." ;
    rdfs:domain sbvr:Bagprojection,
        sbvr:Closedprojection,
        sbvr:Projection,
        sbvr:SetProjection ;
    rdfs:range xsd:anyType .

sbvr:quantification a rdf:Property ;
    rdfs:comment "This is the quantification property or class within the SBVR ontology." ;
    rdfs:domain sbvr:QuantificationIntroducesVariable,
        sbvr:Quantificationscopesoverlogicalformulation .

sbvr:quantity1 a rdf:Property ;
    rdfs:comment "This is the quantity1 property or class within the SBVR ontology." ;
    rdfs:domain sbvr:Quantity1EqualsQuantity2,
        sbvr:Quantity1IsLessThanQuantity2 .

sbvr:Quantity2 a rdf:Property ;
    rdfs:comment "This is the Quantity2 property or class within the SBVR ontology." ;
    rdfs:domain sbvr:Quantity1EqualsQuantity2,
        sbvr:Quantity1IsLessThanQuantity2 .

sbvr:RangedOverConcept a rdf:Property ;
    rdfs:comment "This is the RangedOverConcept property or class within the SBVR ontology." ;
    rdfs:domain sbvr:Auxiliaryvariable,
        sbvr:Variable ;
    rdfs:range xsd:anyType .

sbvr:res a rdf:Property ;
    rdfs:comment "This is the res property or class within the SBVR ontology." ;
    rdfs:domain sbvr:Resissensorymanifestationofsignifier .

sbvr:restrictingFormulation a rdf:Property ;
    rdfs:comment "This is the restrictingFormulation property or class within the SBVR ontology." ;
    rdfs:domain sbvr:Auxiliaryvariable,
        sbvr:Variable ;
    rdfs:range xsd:anyType .

sbvr:scopeFormulation a rdf:Property ;
    rdfs:comment "This is the scopeFormulation property or class within the SBVR ontology." ;
    rdfs:domain sbvr:AtLeastNQuantification,
        sbvr:AtMostNQuantification,
        sbvr:AtMostOneQuantification,
        sbvr:ExactlyNQuantification,
        sbvr:ExactlyOneQuantification,
        sbvr:ExistentialQuantification,
        sbvr:NumericrangeQuantification,
        sbvr:UniversalQuantification ;
    rdfs:range xsd:anyType .

sbvr:semanticFormulation a rdf:Property ;
    rdfs:comment "This is the semanticFormulation property or class within the SBVR ontology." ;
    rdfs:domain sbvr:Variableisfreewithinsemanticformulation .

sbvr:servesAsDesignation a rdf:Property ;
    rdfs:comment "This is the servesAsDesignation property or class within the SBVR ontology." ;
    rdfs:domain sbvr:AdoptedDefinition,
        sbvr:Definitedescription,
        sbvr:Definition,
        sbvr:Extensionaldefinition,
        sbvr:IntensionalDefinition,
        sbvr:Owneddefinition ;
    rdfs:range xsd:boolean .

sbvr:set a rdf:Property ;
    rdfs:comment "This is the set property or class within the SBVR ontology." ;
    rdfs:domain sbvr:Sethascardinality .

sbvr:signifier a rdf:Property ;
    rdfs:comment "Expression that is a linguistic unit or pattern, such as a succession of speech sounds, written symbols or gestures, used in a designation of a concept",
        "This is the signifier property or class within the SBVR ontology." ;
    rdfs:domain sbvr:Designation,
        sbvr:DesignationHasSignifier,
        sbvr:Icon,
        sbvr:Name,
        sbvr:Nonverbaldesignation,
        sbvr:Placeholder,
        sbvr:Preferreddesignation,
        sbvr:Prohibiteddesignation,
        sbvr:Resissensorymanifestationofsignifier,
        sbvr:Speechcommunityregulatesitsusageofsignifier,
        sbvr:Term,
        sbvr:VerbConceptRoledesignation,
        sbvr:Verbsymbol ;
    rdfs:range xsd:anyType .

sbvr:simplyUsedRole a rdf:Property ;
    rdfs:comment "This is the simplyUsedRole property or class within the SBVR ontology." ;
    rdfs:domain sbvr:ReferenceScheme ;
    rdfs:range xsd:anyType .

sbvr:startingCharacterPosition a rdf:Property ;
    rdfs:comment "This is the startingCharacterPosition property or class within the SBVR ontology." ;
    rdfs:domain sbvr:Placeholder,
        sbvr:Placeholderisatstartingcharacterposition ;
    rdfs:range xsd:anyType .

sbvr:subcommunity a rdf:Property ;
    rdfs:comment "This is the subcommunity property or class within the SBVR ontology." ;
    rdfs:domain sbvr:Communityhassubcommunity,
        sbvr:Semanticcommunity,
        sbvr:Speechcommunity ;
    rdfs:range xsd:anyType .

sbvr:subjectConcept a rdf:Property ;
    rdfs:comment "This is the subjectConcept property or class within the SBVR ontology." ;
    rdfs:domain sbvr:AttributiveNamespaceIsForSubjectConcept .

sbvr:thing1 a rdf:Property ;
    rdfs:comment "This is the thing1 property or class within the SBVR ontology.",
        "anything perceivable or conceivable" ;
    rdfs:domain sbvr:Thing1isthing2 .

sbvr:thing2 a rdf:Property ;
    rdfs:comment "This is the thing2 property or class within the SBVR ontology.",
        "anything perceivable or conceivable" ;
    rdfs:domain sbvr:Thing1isthing2 .

sbvr:value a rdf:Property ;
    rdfs:comment "This is the value property or class within the SBVR ontology." ;
    rdfs:domain sbvr:Integer,
        sbvr:NonNegativeInteger,
        sbvr:PositiveInteger,
        sbvr:Text,
        sbvr:URI ;
    rdfs:range xsd:integer,
        xsd:string .

sbvr:VerbConceptObjectification a rdf:Property ;
    rdfs:comment "This is the verbConceptObjectification property or class within the SBVR ontology." ;
    rdfs:domain sbvr:Association,
        sbvr:Binaryverbconcept,
        sbvr:Characteristic,
        sbvr:GeneralVerbConcept,
        sbvr:PartitiveVerbConcept,
        sbvr:PropertyAssociation,
        sbvr:Unitaryverbconcept,
        sbvr:VerbConcept ;
    rdfs:range xsd:anyType .

sbvr:vocabulary1 a rdf:Property ;
    rdfs:comment "This is the vocabulary1 property or class within the SBVR ontology." ;
    rdfs:domain sbvr:Vocabulary1IncorporatesVocabulary2 .

sbvr:vocabulary2 a rdf:Property ;
    rdfs:comment "This is the vocabulary2 property or class within the SBVR ontology." ;
    rdfs:domain sbvr:Vocabulary1IncorporatesVocabulary2 .

sbvr:Authority a rdf:Property,
        owl:Class ;
    rdfs:label "authority" ;
    rdfs:comment "This is the authority property or class within the SBVR ontology." ;
    rdfs:domain sbvr:AuthorityAuthorsGuidanceStatement,
        sbvr:AuthorityDefinesElementofGuidance,
        sbvr:Elementofguidanceisinthejurisdictionofauthority .

sbvr:Bodyofsharedconcepts a rdf:Property,
        owl:Class ;
    rdfs:label "bodyOfSharedConcepts" ;
    rdfs:comment "This is the bodyOfSharedConcepts property or class within the SBVR ontology." ;
    rdfs:domain sbvr:BodyOfSharedConceptsIncludesConcept,
        sbvr:Bodyofsharedmeaningsincludesbodyofsharedconcepts .

sbvr:Bodyofsharedguidance a rdf:Property,
        owl:Class ;
    rdfs:label "bodyOfSharedGuidance" ;
    rdfs:comment "This is the bodyOfSharedGuidance property or class within the SBVR ontology." ;
    rdfs:domain sbvr:Bodyofsharedguidanceincludeselementofguidance,
        sbvr:BodyOfSharedGuidanceIncludesRuleSet,
        sbvr:BodyOfSharedMeaningsIncludesBodyOfSharedGuidance .

sbvr:Categorizationscheme a rdf:Property,
        owl:Class ;
    rdfs:label "categorizationScheme" ;
    rdfs:comment "This is the categorizationScheme property or class within the SBVR ontology." ;
    rdfs:domain sbvr:Categorizationschemecontainscategory,
        sbvr:Categorizationschemeisforgeneralconcept,
        sbvr:Categorizationtype,
        sbvr:Characteristictype,
        sbvr:Concepttype,
        sbvr:Fundamentalconcept,
        sbvr:GeneralConcept,
        sbvr:LogicalFormulationKind,
        sbvr:SituationalRole ;
    rdfs:range xsd:anyType .

sbvr:Closedlogicalformulation a rdf:Property,
        owl:Class ;
    rdfs:label "closedLogicalFormulation" ;
    rdfs:comment "This is the closedLogicalFormulation property or class within the SBVR ontology." ;
    rdfs:domain sbvr:Closedlogicalformulationformalizesstatement,
        sbvr:Closedlogicalformulationmeansproposition .

sbvr:ElementsOfConceptSystemStructure a owl:Class ;
    rdfs:label "ElementsOfConceptSystemStructure" ;
    rdfs:comment "This is the ElementsOfConceptSystemStructure property or class within the SBVR ontology." .

sbvr:Enforcementlevel a rdf:Property,
        owl:Class ;
    rdfs:label "enforcementLevel" ;
    rdfs:comment "This is the enforcementLevel property or class within the SBVR ontology." ;
    rdfs:domain sbvr:BehavioralBusinessRule,
        sbvr:BehavioralBusinessRuleHasEnforcementLevel ;
    rdfs:range xsd:anyType .

sbvr:Instantiationformulation a rdf:Property,
        owl:Class ;
    rdfs:label "instantiationFormulation" ;
    rdfs:comment "This is the instantiationFormulation property or class within the SBVR ontology." ;
    rdfs:domain sbvr:Instantiationformulationbindstobindabletarget,
        sbvr:Instantiationformulationconsidersconcept .

sbvr:Language a rdf:Property,
        owl:Class ;
    rdfs:label "language" ;
    rdfs:comment "This is the language property or class within the SBVR ontology." ;
    rdfs:domain sbvr:Speechcommunityuseslanguage,
        sbvr:vocabularyIsExpressedInLanguage,
        sbvr:VocabularyNamespaceIsForlanguage .

sbvr:Necessityformulation a owl:Class ;
    rdfs:label "necessityFormulation" ;
    rdfs:comment "This is the necessityFormulation property or class within the SBVR ontology." .

sbvr:Objectification a rdf:Property,
        owl:Class ;
    rdfs:label "objectification" ;
    rdfs:comment "This is the objectification property or class within the SBVR ontology." ;
    rdfs:domain sbvr:Objectificationbindstobindabletarget,
        sbvr:Objectificationconsiderslogicalformulation .

sbvr:Obligationformulation a owl:Class ;
    rdfs:label "obligationFormulation" ;
    rdfs:comment "This is the obligationFormulation property or class within the SBVR ontology." .

sbvr:Permissibilityformulation a owl:Class ;
    rdfs:label "permissibilityFormulation" ;
    rdfs:comment "This is the permissibilityFormulation property or class within the SBVR ontology." .

sbvr:Possibilityformulation a owl:Class ;
    rdfs:label "possibilityFormulation" ;
    rdfs:comment "This is the possibilityFormulation property or class within the SBVR ontology." .

sbvr:Property a owl:Class ;
    rdfs:label "property" ;
    rdfs:comment "This is the property property or class within the SBVR ontology." .

sbvr:Propositionnominalization a rdf:Property,
        owl:Class ;
    rdfs:label "propositionNominalization" ;
    rdfs:comment "This is the propositionNominalization property or class within the SBVR ontology." ;
    rdfs:domain sbvr:Propositionnominalizationbindstobindabletarget,
        sbvr:Propositionnominalizationconsiderslogicalformulation .

sbvr:RepresentationFormality a owl:Class ;
    rdfs:label "RepresentationFormality" ;
    rdfs:comment "This is the RepresentationFormality property or class within the SBVR ontology." .

sbvr:Rolebinding a rdf:Property,
        owl:Class ;
    rdfs:label "roleBinding" ;
    rdfs:comment "This is the roleBinding property or class within the SBVR ontology." ;
    rdfs:domain sbvr:Atomicformulation,
        sbvr:Rolebindingbindstobindabletarget,
        sbvr:Rolebindingoccursinatomicformulation,
        sbvr:VerbConceptRole,
        sbvr:VerbConceptRoleHasRolebinding ;
    rdfs:range xsd:anyType .

sbvr:Segmentation a owl:Class ;
    rdfs:label "segmentation" ;
    rdfs:comment "This is the segmentation property or class within the SBVR ontology." .

sbvr:Stateofaffairs a rdf:Property,
        owl:Class ;
    rdfs:label "stateOfAffairs" ;
    rdfs:comment "This is the stateOfAffairs property or class within the SBVR ontology." ;
    rdfs:domain sbvr:Elementofguidanceacknowledgesaspossiblestateofaffairs,
        sbvr:Elementofguidancenecessitatesstateofaffairs,
        sbvr:Elementofguidancepermitsstateofaffairs .

sbvr:Subjectfield a rdf:Property,
        owl:Class ;
    rdfs:label "subjectField" ;
    rdfs:comment "This is the subjectField property or class within the SBVR ontology." ;
    rdfs:domain sbvr:Representationisinsubjectfield,
        sbvr:VocabularyNamespaceisspecifictosubjectfield .

sbvr:Viewpoint a owl:Class ;
    rdfs:label "viewpoint" ;
    rdfs:comment "This is the viewpoint property or class within the SBVR ontology." .

sbvr:AdviceIsDerivedFromBusinessPolicy a owl:Class ;
    rdfs:label "AdviceIsDerivedFromBusinessPolicy" ;
    rdfs:comment "This is the AdviceIsDerivedFromBusinessPolicy property or class within the SBVR ontology." .

sbvr:Aggregationformulation a owl:Class ;
    rdfs:label "aggregationFormulation" ;
    rdfs:comment "This is the aggregationFormulation property or class within the SBVR ontology." .

sbvr:Answernominalization a owl:Class ;
    rdfs:label "answerNominalization" ;
    rdfs:comment "This is the answerNominalization property or class within the SBVR ontology." .

sbvr:AtLeastNQuantificationHasMinimumCardinality a owl:Class ;
    rdfs:label "AtLeastNQuantificationHasMinimumCardinality" ;
    rdfs:comment "This is the AtLeastNQuantificationHasMinimumCardinality property or class within the SBVR ontology." .

sbvr:AtMostNQuantificationHasMaximumCardinality a owl:Class ;
    rdfs:label "AtMostNQuantificationHasMaximumCardinality" ;
    rdfs:comment "This is the AtMostNQuantificationHasMaximumCardinality property or class within the SBVR ontology." .

sbvr:Atomicformulation a rdf:Property,
        owl:Class ;
    rdfs:label "atomicFormulation" ;
    rdfs:comment "This is the atomicFormulation property or class within the SBVR ontology." ;
    rdfs:domain sbvr:Atomicformulationisbasedonverbconcept,
        sbvr:Rolebindingoccursinatomicformulation .

sbvr:Atomicformulationisbasedonverbconcept a owl:Class ;
    rdfs:label "atomicFormulationIsBasedOnVerbConcept" ;
    rdfs:comment "This is the atomicFormulationIsBasedOnVerbConcept property or class within the SBVR ontology." .

sbvr:Attributivenamespace a rdf:Property,
        owl:Class ;
    rdfs:label "attributiveNamespace" ;
    rdfs:comment "This is the attributiveNamespace property or class within the SBVR ontology." ;
    rdfs:domain sbvr:Association,
        sbvr:AttributiveNamespaceIsForSubjectConcept,
        sbvr:AttributiveNamespaceIsWithInVocabularyNamespace,
        sbvr:Binaryverbconcept,
        sbvr:Categorizationtype,
        sbvr:Characteristic,
        sbvr:Characteristictype,
        sbvr:Conceptofthingascomposite,
        sbvr:ConceptOfThingAsContinuant,
        sbvr:ConceptOfThingAsDeveloped,
        sbvr:Conceptofthingasoccurrent,
        sbvr:Conceptofthingasprimitive,
        sbvr:Conceptofthingasunitary,
        sbvr:Conceptofthingexistingdependently,
        sbvr:Conceptofthingexistingindependently,
        sbvr:Concepttype,
        sbvr:Contextualizedconcept,
        sbvr:Derivableconcept,
        sbvr:Facet,
        sbvr:Fundamentalconcept,
        sbvr:GeneralConcept,
        sbvr:GeneralVerbConcept,
        sbvr:IndividualNounConcept,
        sbvr:Integer,
        sbvr:LogicalFormulationKind,
        sbvr:NonNegativeInteger,
        sbvr:NounConcept,
        sbvr:Number,
        sbvr:PartitiveVerbConcept,
        sbvr:PositiveInteger,
        sbvr:PropertyAssociation,
        sbvr:Quantity,
        sbvr:Role,
        sbvr:SituationalRole,
        sbvr:Unitaryverbconcept,
        sbvr:VerbConcept,
        sbvr:VerbConceptRole ;
    rdfs:range xsd:anyType .

sbvr:AttributiveNamespaceIsForSubjectConcept a owl:Class ;
    rdfs:label "attributiveNamespaceIsForSubjectConcept" ;
    rdfs:comment "This is the attributiveNamespaceIsForSubjectConcept property or class within the SBVR ontology." .

sbvr:AttributiveNamespaceIsWithInVocabularyNamespace a owl:Class ;
    rdfs:label "AttributiveNamespaceIsWithInVocabularyNamespace" ;
    rdfs:comment "This is the AttributiveNamespaceIsWithInVocabularyNamespace property or class within the SBVR ontology." .

sbvr:AuthorityAuthorsGuidanceStatement a owl:Class ;
    rdfs:label "AuthorityAuthorsGuidanceStatement" ;
    rdfs:comment "This is the AuthorityAuthorsGuidanceStatement property or class within the SBVR ontology." .

sbvr:AuthorityDefinesElementofGuidance a owl:Class ;
    rdfs:label "AuthorityDefinesElementofGuidance" ;
    rdfs:comment "This is the AuthorityDefinesElementofGuidance property or class within the SBVR ontology." .

sbvr:BehavioralBusinessRuleHasEnforcementLevel a owl:Class ;
    rdfs:label "BehavioralBusinessRuleHasEnforcementLevel" ;
    rdfs:comment "This is the BehavioralBusinessRuleHasEnforcementLevel property or class within the SBVR ontology." .

sbvr:BinaryLogicalOperationHasLogicalOperand1 a owl:Class ;
    rdfs:label "BinaryLogicalOperationHasLogicalOperand1" ;
    rdfs:comment "This is the BinaryLogicalOperationHasLogicalOperand1 property or class within the SBVR ontology." .

sbvr:BinaryLogicalOperationHasLogicalOperand2 a owl:Class ;
    rdfs:label "BinaryLogicalOperationHasLogicalOperand2" ;
    rdfs:comment "This is the BinaryLogicalOperationHasLogicalOperand2 property or class within the SBVR ontology." .

sbvr:BodyOfSharedConceptsIncludesConcept a owl:Class ;
    rdfs:label "BodyOfSharedConceptsIncludesConcept" ;
    rdfs:comment "This is the BodyOfSharedConceptsIncludesConcept property or class within the SBVR ontology." .

sbvr:Bodyofsharedguidanceincludeselementofguidance a owl:Class ;
    rdfs:label "bodyOfSharedGuidanceIncludesElementOfGuidance" ;
    rdfs:comment "This is the bodyOfSharedGuidanceIncludesElementOfGuidance property or class within the SBVR ontology." .

sbvr:BodyOfSharedGuidanceIncludesRuleSet a owl:Class ;
    rdfs:label "BodyOfSharedGuidanceIncludesRuleSet" ;
    rdfs:comment "This is the BodyOfSharedGuidanceIncludesRuleSet property or class within the SBVR ontology." .

sbvr:Bodyofsharedmeanings1containsbodyofsharedmeanings2 a owl:Class ;
    rdfs:label "bodyOfSharedMeanings1ContainsBodyOfSharedMeanings2" ;
    rdfs:comment "This is the bodyOfSharedMeanings1ContainsBodyOfSharedMeanings2 property or class within the SBVR ontology." .

sbvr:Bodyofsharedmeaningsincludesbodyofsharedconcepts a owl:Class ;
    rdfs:label "bodyOfSharedMeaningsIncludesBodyOfSharedConcepts" ;
    rdfs:comment "This is the bodyOfSharedMeaningsIncludesBodyOfSharedConcepts property or class within the SBVR ontology." .

sbvr:BodyOfSharedMeaningsIncludesBodyOfSharedGuidance a owl:Class ;
    rdfs:label "BodyOfSharedMeaningsIncludesBodyOfSharedGuidance" ;
    rdfs:comment "This is the BodyOfSharedMeaningsIncludesBodyOfSharedGuidance property or class within the SBVR ontology." .

sbvr:Bodyofsharedmeaningsunitessemanticcommunity a owl:Class ;
    rdfs:label "bodyOfSharedMeaningsUnitesSemanticCommunity" ;
    rdfs:comment "This is the bodyOfSharedMeaningsUnitesSemanticCommunity property or class within the SBVR ontology." .

sbvr:Businessruleisderivedfrombusinesspolicy a owl:Class ;
    rdfs:label "businessRuleIsDerivedFromBusinessPolicy" ;
    rdfs:comment "This is the businessRuleIsDerivedFromBusinessPolicy property or class within the SBVR ontology." .

sbvr:Categorizationschemecontainscategory a owl:Class ;
    rdfs:label "categorizationSchemeContainsCategory" ;
    rdfs:comment "This is the categorizationSchemeContainsCategory property or class within the SBVR ontology." .

sbvr:Categorizationschemeisforgeneralconcept a owl:Class ;
    rdfs:label "categorizationSchemeIsForGeneralConcept" ;
    rdfs:comment "This is the categorizationSchemeIsForGeneralConcept property or class within the SBVR ontology." .

sbvr:Categorizationtypeisforgeneralconcept a owl:Class ;
    rdfs:label "categorizationTypeIsForGeneralConcept" ;
    rdfs:comment "This is the categorizationTypeIsForGeneralConcept property or class within the SBVR ontology." .

sbvr:Closedlogicalformulationformalizesstatement a owl:Class ;
    rdfs:label "closedLogicalFormulationFormalizesStatement" ;
    rdfs:comment "This is the closedLogicalFormulationFormalizesStatement property or class within the SBVR ontology." .

sbvr:Closedlogicalformulationmeansproposition a owl:Class ;
    rdfs:label "closedLogicalFormulationMeansProposition" ;
    rdfs:comment "This is the closedLogicalFormulationMeansProposition property or class within the SBVR ontology." .

sbvr:ClosedprojectiondefinesNounConcept a owl:Class ;
    rdfs:label "closedProjectionDefinesNounConcept" ;
    rdfs:comment "This is the closedProjectionDefinesNounConcept property or class within the SBVR ontology." .

sbvr:Closedprojectiondefinesverbconcept a owl:Class ;
    rdfs:label "closedProjectionDefinesVerbConcept" ;
    rdfs:comment "This is the closedProjectionDefinesVerbConcept property or class within the SBVR ontology." .

sbvr:Closedprojectionformalizesdefinition a owl:Class ;
    rdfs:label "closedProjectionFormalizesDefinition" ;
    rdfs:comment "This is the closedProjectionFormalizesDefinition property or class within the SBVR ontology." .

sbvr:Closedprojectionmeansquestion a owl:Class ;
    rdfs:label "closedProjectionMeansQuestion" ;
    rdfs:comment "This is the closedProjectionMeansQuestion property or class within the SBVR ontology." .

sbvr:Closedsemanticformulationformulatesmeaning a owl:Class ;
    rdfs:label "closedSemanticFormulationFormulatesMeaning" ;
    rdfs:comment "This is the closedSemanticFormulationFormulatesMeaning property or class within the SBVR ontology." .

sbvr:Communicationcontentiscomposedofrepresentation a owl:Class ;
    rdfs:label "communicationContentIsComposedOfRepresentation" ;
    rdfs:comment "This is the communicationContentIsComposedOfRepresentation property or class within the SBVR ontology." .

sbvr:Communityhassubcommunity a owl:Class ;
    rdfs:label "communityHasSubcommunity" ;
    rdfs:comment "This is the communityHasSubcommunity property or class within the SBVR ontology." .

sbvr:CommunityHasUri a owl:Class ;
    rdfs:label "CommunityHasUri" ;
    rdfs:comment "This is the CommunityHasUri property or class within the SBVR ontology." .

sbvr:Concept1iscoextensivewithconcept2 a owl:Class ;
    rdfs:label "concept1IsCoextensiveWithConcept2" ;
    rdfs:comment "This is the concept1IsCoextensiveWithConcept2 property or class within the SBVR ontology." .

sbvr:Concept1specializesconcept2 a owl:Class ;
    rdfs:label "concept1SpecializesConcept2" ;
    rdfs:comment "This is the concept1SpecializesConcept2 property or class within the SBVR ontology." .

sbvr:ConceptHasDefinition a owl:Class ;
    rdfs:label "ConceptHasDefinition" ;
    rdfs:comment "This is the ConceptHasDefinition property or class within the SBVR ontology." .

sbvr:ConceptHasDesignation a owl:Class ;
    rdfs:label "ConceptHasDesignation" ;
    rdfs:comment "This is the ConceptHasDesignation property or class within the SBVR ontology." .

sbvr:ConceptHasExtension a owl:Class ;
    rdfs:label "ConceptHasExtension" ;
    rdfs:comment "This is the ConceptHasExtension property or class within the SBVR ontology." .

sbvr:ConceptHasFacet a owl:Class ;
    rdfs:label "ConceptHasFacet" ;
    rdfs:comment "This is the ConceptHasFacet property or class within the SBVR ontology." .

sbvr:ConceptHasImpliedCharacteristic a owl:Class ;
    rdfs:label "ConceptHasImpliedCharacteristic" ;
    rdfs:comment "This is the ConceptHasImpliedCharacteristic property or class within the SBVR ontology." .

sbvr:ConceptHasInstance a owl:Class ;
    rdfs:label "ConceptHasInstance" ;
    rdfs:comment "This is the ConceptHasInstance property or class within the SBVR ontology." .

sbvr:ConceptHasNecessaryCharacteristic a owl:Class ;
    rdfs:label "ConceptHasNecessaryCharacteristic" ;
    rdfs:comment "This is the ConceptHasNecessaryCharacteristic property or class within the SBVR ontology." .

sbvr:ConceptIncorporatesCharacteristic a owl:Class ;
    rdfs:label "ConceptIncorporatesCharacteristic" ;
    rdfs:comment "This is the ConceptIncorporatesCharacteristic property or class within the SBVR ontology." .

sbvr:DescriptionPortraysMeaning a owl:Class ;
    rdfs:label "DescriptionPortraysMeaning" ;
    rdfs:comment "This is the DescriptionPortraysMeaning property or class within the SBVR ontology." .

sbvr:DescriptiveExampleIllustratesMeaning a owl:Class ;
    rdfs:label "DescriptiveExampleIllustratesMeaning" ;
    rdfs:comment "This is the DescriptiveExampleIllustratesMeaning property or class within the SBVR ontology." .

sbvr:DesignationHasSignifier a owl:Class ;
    rdfs:label "DesignationHasSignifier" ;
    rdfs:comment "This is the DesignationHasSignifier property or class within the SBVR ontology." .

sbvr:designationIsInNamespace a rdf:Property ;
    rdfs:label "designationIsInNamespace" ;
    rdfs:comment "This is the designationIsInNamespace property or class within the SBVR ontology." .

sbvr:Elementofguidanceacknowledgesaspossiblestateofaffairs a owl:Class ;
    rdfs:label "elementOfGuidanceAcknowledgesAsPossibleStateOfAffairs" ;
    rdfs:comment "This is the elementOfGuidanceAcknowledgesAsPossibleStateOfAffairs property or class within the SBVR ontology." .

sbvr:Elementofguidanceisinthejurisdictionofauthority a owl:Class ;
    rdfs:label "elementOfGuidanceIsInTheJurisdictionOfAuthority" ;
    rdfs:comment "This is the elementOfGuidanceIsInTheJurisdictionOfAuthority property or class within the SBVR ontology." .

sbvr:Elementofguidancenecessitatesstateofaffairs a owl:Class ;
    rdfs:label "elementOfGuidanceNecessitatesStateOfAffairs" ;
    rdfs:comment "This is the elementOfGuidanceNecessitatesStateOfAffairs property or class within the SBVR ontology." .

sbvr:Elementofguidancepermitsstateofaffairs a owl:Class ;
    rdfs:label "elementOfGuidancePermitsStateOfAffairs" ;
    rdfs:comment "This is the elementOfGuidancePermitsStateOfAffairs property or class within the SBVR ontology." .

sbvr:ExactlyNQuantificationHasCardinality a owl:Class ;
    rdfs:label "ExactlyNQuantificationHasCardinality" ;
    rdfs:comment "This is the ExactlyNQuantificationHasCardinality property or class within the SBVR ontology." .

sbvr:Expressionisunambiguoustospeechcommunity a owl:Class ;
    rdfs:label "expressionIsUnambiguousToSpeechCommunity" ;
    rdfs:comment "This is the expressionIsUnambiguousToSpeechCommunity property or class within the SBVR ontology." .

sbvr:Expressionrepresentsmeaning a owl:Class ;
    rdfs:label "expressionRepresentsMeaning" ;
    rdfs:comment "This is the expressionRepresentsMeaning property or class within the SBVR ontology." .

sbvr:GeneralConceptobjectifiesverbconcept a owl:Class ;
    rdfs:label "generalConceptObjectifiesVerbConcept" ;
    rdfs:comment "This is the generalConceptObjectifiesVerbConcept property or class within the SBVR ontology." .

sbvr:Implicationhasantecedent a owl:Class ;
    rdfs:label "implicationHasAntecedent" ;
    rdfs:comment "This is the implicationHasAntecedent property or class within the SBVR ontology." .

sbvr:Implicationhasconsequent a owl:Class ;
    rdfs:label "implicationHasConsequent" ;
    rdfs:comment "This is the implicationHasConsequent property or class within the SBVR ontology." .

sbvr:Instantiationformulationbindstobindabletarget a owl:Class ;
    rdfs:label "instantiationFormulationBindsToBindableTarget" ;
    rdfs:comment "This is the instantiationFormulationBindsToBindableTarget property or class within the SBVR ontology." .

sbvr:Instantiationformulationconsidersconcept a owl:Class ;
    rdfs:label "instantiationFormulationConsidersConcept" ;
    rdfs:comment "This is the instantiationFormulationConsidersConcept property or class within the SBVR ontology." .

sbvr:IntensionalDefinitionusesdelimitingcharacteristic a owl:Class ;
    rdfs:label "IntensionalDefinitionUsesDelimitingCharacteristic" ;
    rdfs:comment "This is the IntensionalDefinitionUsesDelimitingCharacteristic property or class within the SBVR ontology." .

sbvr:Logicalformulationconstrainsprojection a owl:Class ;
    rdfs:label "logicalFormulationConstrainsProjection" ;
    rdfs:comment "This is the logicalFormulationConstrainsProjection property or class within the SBVR ontology." .

sbvr:Logicalformulationrestrictsvariable a owl:Class ;
    rdfs:label "logicalFormulationRestrictsVariable" ;
    rdfs:comment "This is the logicalFormulationRestrictsVariable property or class within the SBVR ontology." .

sbvr:Logicalnegation a owl:Class ;
    rdfs:label "logicalNegation" ;
    rdfs:comment "This is the logicalNegation property or class within the SBVR ontology." .

sbvr:Logicaloperationhaslogicaloperand a owl:Class ;
    rdfs:label "logicalOperationHasLogicalOperand" ;
    rdfs:comment "This is the logicalOperationHasLogicalOperand property or class within the SBVR ontology." .

sbvr:Modalformulationembedslogicalformulation a owl:Class ;
    rdfs:label "modalFormulationEmbedsLogicalFormulation" ;
    rdfs:comment "This is the modalFormulationEmbedsLogicalFormulation property or class within the SBVR ontology." .

sbvr:Namespace a rdf:Property,
        owl:Class ;
    rdfs:label "namespace" ;
    rdfs:comment "This is the namespace property or class within the SBVR ontology." ;
    rdfs:domain sbvr:designationIsInNamespace,
        sbvr:namespaceHasURI,
        sbvr:VerbConceptWordingIsInNamespace .

sbvr:Namespace1incorporatesnamespace2 a owl:Class ;
    rdfs:label "namespace1IncorporatesNamespace2" ;
    rdfs:comment "This is the namespace1IncorporatesNamespace2 property or class within the SBVR ontology." .

sbvr:namespaceHasURI a owl:Class, 
        rdfs:Property ;
    rdfs:label "NamespaceHasURI" ;
    rdfs:comment "This is the NamespaceHasURI property or class within the SBVR ontology." .

sbvr:NoteCommentsOnMeaning a owl:Class ;
    rdfs:label "NoteCommentsOnMeaning" ;
    rdfs:comment "This is the NoteCommentsOnMeaning property or class within the SBVR ontology." .

sbvr:NounConceptnominalization a owl:Class ;
    rdfs:label "NounConceptNominalization" ;
    rdfs:comment "This is the NounConceptNominalization property or class within the SBVR ontology." .

sbvr:NumericrangeQuantificationhasmaximumcardinality a owl:Class ;
    rdfs:label "numericRangeQuantificationHasMaximumCardinality" ;
    rdfs:comment "This is the numericRangeQuantificationHasMaximumCardinality property or class within the SBVR ontology." .

sbvr:NumericrangeQuantificationhasminimumcardinality a owl:Class ;
    rdfs:label "numericRangeQuantificationHasMinimumCardinality" ;
    rdfs:comment "This is the numericRangeQuantificationHasMinimumCardinality property or class within the SBVR ontology." .

sbvr:Objectificationbindstobindabletarget a owl:Class ;
    rdfs:label "objectificationBindsToBindableTarget" ;
    rdfs:comment "This is the objectificationBindsToBindableTarget property or class within the SBVR ontology." .

sbvr:Objectificationconsiderslogicalformulation a owl:Class ;
    rdfs:label "objectificationConsidersLogicalFormulation" ;
    rdfs:comment "This is the objectificationConsidersLogicalFormulation property or class within the SBVR ontology." .

sbvr:Placeholderisatstartingcharacterposition a owl:Class ;
    rdfs:label "placeholderIsAtStartingCharacterPosition" ;
    rdfs:comment "This is the placeholderIsAtStartingCharacterPosition property or class within the SBVR ontology." .

sbvr:Placeholderisinverbconceptwording a owl:Class ;
    rdfs:label "placeholderIsInVerbConceptWording" ;
    rdfs:comment "This is the placeholderIsInVerbConceptWording property or class within the SBVR ontology." .

sbvr:Placeholderusesdesignation a owl:Class ;
    rdfs:label "placeholderUsesDesignation" ;
    rdfs:comment "This is the placeholderUsesDesignation property or class within the SBVR ontology." .

sbvr:Projectingformulationbindstobindabletarget a owl:Class ;
    rdfs:label "projectingFormulationBindsToBindableTarget" ;
    rdfs:comment "This is the projectingFormulationBindsToBindableTarget property or class within the SBVR ontology." .

sbvr:Projectingformulationhasprojection a owl:Class ;
    rdfs:label "projectingFormulationHasProjection" ;
    rdfs:comment "This is the projectingFormulationHasProjection property or class within the SBVR ontology." .

sbvr:Projectionhasauxiliaryvariable a owl:Class ;
    rdfs:label "projectionHasAuxiliaryVariable" ;
    rdfs:comment "This is the projectionHasAuxiliaryVariable property or class within the SBVR ontology." .

sbvr:Projectionisonvariable a owl:Class ;
    rdfs:label "projectionIsOnVariable" ;
    rdfs:comment "This is the projectionIsOnVariable property or class within the SBVR ontology." .

sbvr:Propositionisbasedonverbconcept a owl:Class ;
    rdfs:label "propositionIsBasedOnVerbConcept" ;
    rdfs:comment "This is the propositionIsBasedOnVerbConcept property or class within the SBVR ontology." .

sbvr:Propositionnominalizationbindstobindabletarget a owl:Class ;
    rdfs:label "propositionNominalizationBindsToBindableTarget" ;
    rdfs:comment "This is the propositionNominalizationBindsToBindableTarget property or class within the SBVR ontology." .

sbvr:Propositionnominalizationconsiderslogicalformulation a owl:Class ;
    rdfs:label "propositionNominalizationConsidersLogicalFormulation" ;
    rdfs:comment "This is the propositionNominalizationConsidersLogicalFormulation property or class within the SBVR ontology." .

sbvr:QuantificationIntroducesVariable a owl:Class ;
    rdfs:label "QuantificationIntroducesVariable" ;
    rdfs:comment "This is the QuantificationIntroducesVariable property or class within the SBVR ontology." .

sbvr:Quantificationscopesoverlogicalformulation a owl:Class ;
    rdfs:label "QuantificationScopesOverLogicalFormulation" ;
    rdfs:comment "This is the QuantificationScopesOverLogicalFormulation property or class within the SBVR ontology." .

sbvr:Quantity1EqualsQuantity2 a owl:Class ;
    rdfs:label "Quantity1EqualsQuantity2" ;
    rdfs:comment "This is the Quantity1EqualsQuantity2 property or class within the SBVR ontology." .

sbvr:Quantity1IsLessThanQuantity2 a owl:Class ;
    rdfs:label "Quantity1IsLessThanQuantity2" ;
    rdfs:comment "This is the Quantity1IsLessThanQuantity2 property or class within the SBVR ontology." .

sbvr:question a rdf:Property,
        owl:Class ;
    rdfs:label "question" ;
    rdfs:comment "This is the question property or class within the SBVR ontology." ;
    rdfs:domain sbvr:Closedprojectionmeansquestion .

sbvr:QuestionNominalization a owl:Class ;
    rdfs:label "QuestionNominalization" ;
    rdfs:comment "This is the QuestionNominalization property or class within the SBVR ontology." .

sbvr:ReferencePointsToInformationSource a owl:Class ;
    rdfs:label "ReferencePointsToInformationSource" ;
    rdfs:comment "This is the ReferencePointsToInformationSource property or class within the SBVR ontology." .

sbvr:ReferenceSchemeextensionallyusesverbconceptrole a owl:Class ;
    rdfs:label "ReferenceSchemeExtensionallyUsesVerbConceptRole" ;
    rdfs:comment "This is the ReferenceSchemeExtensionallyUsesVerbConceptRole property or class within the SBVR ontology." .

sbvr:ReferenceSchemeisforconcept a owl:Class ;
    rdfs:label "ReferenceSchemeIsForConcept" ;
    rdfs:comment "This is the ReferenceSchemeIsForConcept property or class within the SBVR ontology." .

sbvr:ReferenceSchemesimplyusesverbconceptrole a owl:Class ;
    rdfs:label "ReferenceSchemeSimplyUsesVerbConceptRole" ;
    rdfs:comment "This is the ReferenceSchemeSimplyUsesVerbConceptRole property or class within the SBVR ontology." .

sbvr:ReferenceSchemeUsesCharacteristic a owl:Class ;
    rdfs:label "ReferenceSchemeUsesCharacteristic" ;
    rdfs:comment "This is the ReferenceSchemeUsesCharacteristic property or class within the SBVR ontology." .

sbvr:ReferenceSupportsMeaning a owl:Class ;
    rdfs:label "ReferenceSupportsMeaning" ;
    rdfs:comment "This is the ReferenceSupportsMeaning property or class within the SBVR ontology." .

sbvr:RepresentationHasExpression a owl:Class ;
    rdfs:label "RepresentationHasExpression" ;
    rdfs:comment "This is the RepresentationHasExpression property or class within the SBVR ontology." .

sbvr:Representationisindesignationcontext a owl:Class ;
    rdfs:label "representationIsInDesignationContext" ;
    rdfs:comment "This is the representationIsInDesignationContext property or class within the SBVR ontology." .

sbvr:Representationisinsubjectfield a owl:Class ;
    rdfs:label "representationIsInSubjectField" ;
    rdfs:comment "This is the representationIsInSubjectField property or class within the SBVR ontology." .

sbvr:Representationrepresentsmeaning a owl:Class ;
    rdfs:label "representationRepresentsMeaning" ;
    rdfs:comment "This is the representationRepresentsMeaning property or class within the SBVR ontology." .

sbvr:RepresentationUsesVocabulary a owl:Class ;
    rdfs:label "RepresentationUsesVocabulary" ;
    rdfs:comment "This is the RepresentationUsesVocabulary property or class within the SBVR ontology." .

sbvr:Resissensorymanifestationofsignifier a owl:Class ;
    rdfs:label "resIsSensoryManifestationOfSignifier" ;
    rdfs:comment "This is the resIsSensoryManifestationOfSignifier property or class within the SBVR ontology." .

sbvr:Rolebindingbindstobindabletarget a owl:Class ;
    rdfs:label "roleBindingBindsToBindableTarget" ;
    rdfs:comment "This is the roleBindingBindsToBindableTarget property or class within the SBVR ontology." .

sbvr:Rolebindingoccursinatomicformulation a owl:Class ;
    rdfs:label "roleBindingOccursInAtomicFormulation" ;
    rdfs:comment "This is the roleBindingOccursInAtomicFormulation property or class within the SBVR ontology." .

sbvr:RoleRangesOverGeneralConcept a owl:Class ;
    rdfs:label "roleRangesOverGeneralConcept" ;
    rdfs:comment "This is the roleRangesOverGeneralConcept property or class within the SBVR ontology." .

sbvr:Rulebook a owl:Class ;
    rdfs:label "Rulebook" ;
    rdfs:comment "This is the rulebook property or class within the SBVR ontology." ;
    rdfs:domain sbvr:RulebookHasUri .

sbvr:RulebookHasUri a owl:Class ;
    rdfs:label "RulebookHasUri" ;
    rdfs:comment "This is the RulebookHasUri property or class within the SBVR ontology." .

sbvr:RuleSetIncludesElementOfGuidance a owl:Class ;
    rdfs:label "RuleSetIncludesElementOfGuidance" ;
    rdfs:comment "This is the RuleSetIncludesElementOfGuidance property or class within the SBVR ontology." .

sbvr:SbvrRulebook a owl:Class ;
    rdfs:label "SbvrRulebook" ;
    rdfs:comment "This is the SbvrRulebook property or class within the SBVR ontology." .

sbvr:Semanticcommunityhasspeechcommunity a owl:Class ;
    rdfs:label "semanticCommunityHasSpeechCommunity" ;
    rdfs:comment "This is the semanticCommunityHasSpeechCommunity property or class within the SBVR ontology." .

sbvr:Semanticcommunitysharesunderstandingofconcept a owl:Class ;
    rdfs:label "semanticCommunitySharesUnderstandingOfConcept" ;
    rdfs:comment "This is the semanticCommunitySharesUnderstandingOfConcept property or class within the SBVR ontology." .

sbvr:Sethascardinality a owl:Class ;
    rdfs:label "setHasCardinality" ;
    rdfs:comment "This is the setHasCardinality property or class within the SBVR ontology." .

sbvr:Speechcommunitydeterminesspeechcommunityrepresentationset a owl:Class ;
    rdfs:label "speechCommunityDeterminesSpeechCommunityRepresentationSet" ;
    rdfs:comment "This is the speechCommunityDeterminesSpeechCommunityRepresentationSet property or class within the SBVR ontology." .

sbvr:Speechcommunityownsowneddefinition a owl:Class ;
    rdfs:label "speechCommunityOwnsOwnedDefinition" ;
    rdfs:comment "This is the speechCommunityOwnsOwnedDefinition property or class within the SBVR ontology." .

sbvr:Speechcommunityownsvocabulary a owl:Class ;
    rdfs:label "speechCommunityOwnsVocabulary" ;
    rdfs:comment "This is the speechCommunityOwnsVocabulary property or class within the SBVR ontology." .

sbvr:Speechcommunityregulatesitsusageofsignifier a owl:Class ;
    rdfs:label "speechCommunityRegulatesItsUsageOfSignifier" ;
    rdfs:comment "This is the speechCommunityRegulatesItsUsageOfSignifier property or class within the SBVR ontology." .

sbvr:Speechcommunityrepresentationsetincludesrepresentation a owl:Class ;
    rdfs:label "speechCommunityRepresentationSetIncludesRepresentation" ;
    rdfs:comment "This is the speechCommunityRepresentationSetIncludesRepresentation property or class within the SBVR ontology." .

sbvr:Speechcommunityuseslanguage a owl:Class ;
    rdfs:label "speechCommunityUsesLanguage" ;
    rdfs:comment "This is the speechCommunityUsesLanguage property or class within the SBVR ontology." .

sbvr:Speechcommunityusesvocabulary a owl:Class ;
    rdfs:label "speechCommunityUsesVocabulary" ;
    rdfs:comment "This is the speechCommunityUsesVocabulary property or class within the SBVR ontology." .

sbvr:Statementexpressesproposition a owl:Class ;
    rdfs:label "statementExpressesProposition" ;
    rdfs:comment "This is the statementExpressesProposition property or class within the SBVR ontology." .

sbvr:Terminologicaldictionary a rdf:Property,
        owl:Class ;
    rdfs:label "terminologicalDictionary" ;
    rdfs:comment "This is the terminologicalDictionary property or class within the SBVR ontology." ;
    rdfs:domain sbvr:Terminologicaldictionaryexpressesbodyofsharedmeanings,
        sbvr:Terminologicaldictionaryhasuri,
        sbvr:Terminologicaldictionaryincludesrepresentation,
        sbvr:Terminologicaldictionarypresentsvocabulary .

sbvr:Terminologicaldictionaryexpressesbodyofsharedmeanings a owl:Class ;
    rdfs:label "terminologicalDictionaryExpressesBodyOfSharedMeanings" ;
    rdfs:comment "This is the terminologicalDictionaryExpressesBodyOfSharedMeanings property or class within the SBVR ontology." .

sbvr:Terminologicaldictionaryhasuri a owl:Class ;
    rdfs:label "terminologicalDictionaryHasURI" ;
    rdfs:comment "This is the terminologicalDictionaryHasURI property or class within the SBVR ontology." .

sbvr:Terminologicaldictionaryincludesrepresentation a owl:Class ;
    rdfs:label "terminologicalDictionaryIncludesRepresentation" ;
    rdfs:comment "This is the terminologicalDictionaryIncludesRepresentation property or class within the SBVR ontology." .

sbvr:Terminologicaldictionarypresentsvocabulary a owl:Class ;
    rdfs:label "terminologicalDictionaryPresentsVocabulary" ;
    rdfs:comment "This is the terminologicalDictionaryPresentsVocabulary property or class within the SBVR ontology." .

sbvr:Text a owl:Class ;
    rdfs:label "Text" ;
    rdfs:comment "This is the text property or class within the SBVR ontology." .

sbvr:Thing1isthing2 a owl:Class ;
    rdfs:label "Thing1IsThing2" ;
    rdfs:comment "This is the thing1IsThing2 property or class within the SBVR ontology." .

sbvr:URI a rdf:Property,
        owl:Class ;
    rdfs:label "URI" ;
    rdfs:comment "This is the URI property or class within the SBVR ontology." ;
    rdfs:domain sbvr:Attributivenamespace,
        sbvr:CommunityHasUri,
        sbvr:Namespace,
        sbvr:namespaceHasURI,
        sbvr:Rulebook,
        sbvr:RulebookHasUri,
        sbvr:SbvrRulebook,
        sbvr:Semanticcommunity,
        sbvr:Speechcommunity,
        sbvr:Terminologicaldictionary,
        sbvr:Terminologicaldictionaryhasuri,
        sbvr:VocabularyNamespace ;
    rdfs:range xsd:anyType .

sbvr:UniversalQuantification a owl:Class ;
    rdfs:label "universalQuantification" ;
    rdfs:comment "This is the universalQuantification property or class within the SBVR ontology." .

sbvr:Variablehasprojectionposition a owl:Class ;
    rdfs:label "variableHasProjectionPosition" ;
    rdfs:comment "This is the variableHasProjectionPosition property or class within the SBVR ontology." .

sbvr:Variableisfreewithinsemanticformulation a owl:Class ;
    rdfs:label "variableIsFreeWithinSemanticFormulation" ;
    rdfs:comment "This is the variableIsFreeWithinSemanticFormulation property or class within the SBVR ontology." .

sbvr:Variablemapstoverbconceptrole a owl:Class ;
    rdfs:label "variableMapsToVerbConceptRole" ;
    rdfs:comment "This is the variableMapsToVerbConceptRole property or class within the SBVR ontology." .

sbvr:Variablerangesoverconcept a owl:Class ;
    rdfs:label "variableRangesOverConcept" ;
    rdfs:comment "This is the variableRangesOverConcept property or class within the SBVR ontology." .

sbvr:VerbConcepthasverbconceptwording a owl:Class ;
    rdfs:label "verbConceptHasVerbConceptWording" ;
    rdfs:comment "This is the verbConceptHasVerbConceptWording property or class within the SBVR ontology." .

sbvr:VerbConceptnominalization a owl:Class ;
    rdfs:label "verbConceptNominalization" ;
    rdfs:comment "This is the verbConceptNominalization property or class within the SBVR ontology." .

sbvr:VerbConceptRoleHasRolebinding a owl:Class ;
    rdfs:label "verbConceptRoleHasRoleBinding" ;
    rdfs:comment "This is the verbConceptRoleHasRoleBinding property or class within the SBVR ontology." .

sbvr:VerbConceptRoleIsInVerbConcept a owl:Class ;
    rdfs:label "verbConceptRoleIsInVerbConcept" ;
    rdfs:comment "This is the verbConceptRoleIsInVerbConcept property or class within the SBVR ontology." .

sbvr:VerbConceptWordinginCorporatesVerbSymbol a owl:Class ;
    rdfs:label "verbConceptWordingIncorporatesVerbSymbol" ;
    rdfs:comment "This is the verbConceptWordingIncorporatesVerbSymbol property or class within the SBVR ontology." .

sbvr:VerbConceptWordingIsInNamespace a owl:Class ;
    rdfs:label "verbConceptWordingIsInNamespace" ;
    rdfs:comment "This is the verbConceptWordingIsInNamespace property or class within the SBVR ontology." .

sbvr:Vocabulary1IncorporatesVocabulary2 a owl:Class ;
    rdfs:label "Vocabulary1IncorporatesVocabulary2" ;
    rdfs:comment "This is the Vocabulary1IncorporatesVocabulary2 property or class within the SBVR ontology." .

sbvr:Vocabularyisdesignedforspeechcommunity a owl:Class, 
        rdf:Property ;
    rdfs:label "Vocabularyisdesignedforspeechcommunity" ;
    rdfs:comment "This is the Vocabularyisdesignedforspeechcommunity property or class within the SBVR ontology." .

sbvr:vocabularyIsExpressedInLanguage a owl:Class, 
        rdf:Property ;
    rdfs:label "VocabularyIsExpressedInLanguage" ;
    rdfs:comment "This is the VocabularyIsExpressedInLanguage property or class within the SBVR ontology." .

sbvr:Vocabularyisusedtoexpressbodyofsharedmeanings a owl:Class ;
    rdfs:label "vocabularyIsUsedToExpressBodyOfSharedMeanings" ;
    rdfs:comment "This is the vocabularyIsUsedToExpressBodyOfSharedMeanings property or class within the SBVR ontology." .

sbvr:VocabularyNamespace a rdf:Property,
        owl:Class ;
    rdfs:label "VocabularyNamespace" ;
    rdfs:comment "This is the VocabularyNamespace property or class within the SBVR ontology." ;
    rdfs:domain sbvr:AttributiveNamespaceIsWithInVocabularyNamespace,
        sbvr:vocabularyNamespaceIsDerivedFromVocabulary,
        sbvr:VocabularyNamespaceIsForlanguage,
        sbvr:VocabularyNamespaceIsSpecificToDesignationContext,
        sbvr:VocabularyNamespaceisspecifictosubjectfield .

sbvr:vocabularyNamespaceIsDerivedFromVocabulary a owl:Class,
        rdf:Property ;
    rdfs:label "VocabularyNamespaceIsDerivedFromVocabulary" ;
    rdfs:comment "This is the VocabularyNamespaceIsDerivedFromVocabulary property or class within the SBVR ontology." .

sbvr:VocabularyNamespaceIsForlanguage a owl:Class ;
    rdfs:label "VocabularyNamespaceIsForlanguage" ;
    rdfs:comment "This is the VocabularyNamespaceIsForlanguage property or class within the SBVR ontology." .

sbvr:VocabularyNamespaceIsSpecificToDesignationContext a owl:Class ;
    rdfs:label "VocabularyNamespaceIsSpecificToDesignationContext" ;
    rdfs:comment "This is the VocabularyNamespaceIsSpecificToDesignationContext property or class within the SBVR ontology." .

sbvr:VocabularyNamespaceisspecifictosubjectfield a owl:Class ;
    rdfs:label "VocabularyNamespaceIsSpecificToSubjectField" ;
    rdfs:comment "This is the VocabularyNamespaceIsSpecificToSubjectField property or class within the SBVR ontology." .

sbvr:WhetherOrNotFormulationHasConsequent a owl:Class ;
    rdfs:label "WhetherOrNotFormulationHasConsequent" ;
    rdfs:comment "This is the WhetherOrNotFormulationHasConsequent property or class within the SBVR ontology." .

sbvr:WhetherOrNotFormulationHasInconsequent a owl:Class ;
    rdfs:label "WhetherOrNotFormulationHasInconsequent" ;
    rdfs:comment "This is the WhetherOrNotFormulationHasInconsequent property or class within the SBVR ontology." .

sbvr:Advicestatement a owl:Class ;
    rdfs:label "AdviceStatement" ;
    rdfs:comment "This is the AdviceStatement property or class within the SBVR ontology." .

sbvr:AtLeastNQuantification a rdf:Property,
        owl:Class ;
    rdfs:label "AtLeastNQuantification" ;
    rdfs:comment "This is the AtLeastNQuantification property or class within the SBVR ontology." ;
    rdfs:domain sbvr:AtLeastNQuantificationHasMinimumCardinality .

sbvr:AtMostNQuantification a rdf:Property,
        owl:Class ;
    rdfs:label "AtMostNQuantification" ;
    rdfs:comment "This is the AtMostNQuantification property or class within the SBVR ontology." ;
    rdfs:domain sbvr:AtMostNQuantificationHasMaximumCardinality .

sbvr:AtMostOneQuantification a owl:Class ;
    rdfs:label "AtMostOneQuantification" ;
    rdfs:comment "This is the AtMostOneQuantification property or class within the SBVR ontology." .

sbvr:BehavioralBusinessRulestatement a owl:Class ;
    rdfs:label "BehavioralBusinessRuleStatement" ;
    rdfs:comment "This is the BehavioralBusinessRuleStatement property or class within the SBVR ontology." .

sbvr:Bodyofsharedmeanings a rdf:Property,
        owl:Class ;
    rdfs:label "bodyOfSharedMeanings" ;
    rdfs:comment "This is the bodyOfSharedMeanings property or class within the SBVR ontology." ;
    rdfs:domain sbvr:Bodyofsharedmeaningsincludesbodyofsharedconcepts,
        sbvr:BodyOfSharedMeaningsIncludesBodyOfSharedGuidance,
        sbvr:Bodyofsharedmeaningsunitessemanticcommunity,
        sbvr:Terminologicaldictionaryexpressesbodyofsharedmeanings,
        sbvr:Vocabularyisusedtoexpressbodyofsharedmeanings .

sbvr:Businesspolicystatement a owl:Class ;
    rdfs:label "businessPolicyStatement" ;
    rdfs:comment "This is the businessPolicyStatement property or class within the SBVR ontology." .

sbvr:Businessvocabulary a owl:Class ;
    rdfs:label "businessVocabulary" ;
    rdfs:comment "This is the businessVocabulary property or class within the SBVR ontology." .

sbvr:Categorization a owl:Class ;
    rdfs:label "categorization" ;
    rdfs:comment "This is the categorization property or class within the SBVR ontology." .

sbvr:Characterization a owl:Class ;
    rdfs:label "characterization" ;
    rdfs:comment "This is the characterization property or class within the SBVR ontology." .

sbvr:Classification a owl:Class ;
    rdfs:label "classification" ;
    rdfs:comment "This is the classification property or class within the SBVR ontology." .

sbvr:Communicationcontent a rdf:Property,
        owl:Class ;
    rdfs:label "communicationContent" ;
    rdfs:comment "This is the communicationContent property or class within the SBVR ontology." ;
    rdfs:domain sbvr:Communicationcontentiscomposedofrepresentation .

sbvr:Contingencystatement a owl:Class ;
    rdfs:label "contingencyStatement" ;
    rdfs:comment "This is the contingencyStatement property or class within the SBVR ontology." .

sbvr:DefinitionalBusinessRule a owl:Class ;
    rdfs:label "DefinitionalBusinessRule" ;
    rdfs:comment "This is the DefinitionalBusinessRule property or class within the SBVR ontology." .

sbvr:DefinitionalRule a owl:Class ;
    rdfs:label "DefinitionalRule" ;
    rdfs:comment "This is the DefinitionalRule property or class within the SBVR ontology." .

sbvr:DefinitionalRuleStatement a owl:Class ;
    rdfs:label "DefinitionalRuleStatement" ;
    rdfs:comment "This is the DefinitionalRuleStatement property or class within the SBVR ontology." .

sbvr:Description a rdf:Property,
        owl:Class ;
    rdfs:label "description" ;
    rdfs:comment "This is the description property or class within the SBVR ontology." ;
    rdfs:domain sbvr:DescriptionPortraysMeaning .

sbvr:Descriptiveexample a rdf:Property,
        owl:Class ;
    rdfs:label "descriptiveExample" ;
    rdfs:comment "This is the descriptiveExample property or class within the SBVR ontology." ;
    rdfs:domain sbvr:DescriptiveExampleIllustratesMeaning .

sbvr:ExactlyNQuantification a rdf:Property,
        owl:Class ;
    rdfs:label "ExactlyNQuantification" ;
    rdfs:comment "This is the ExactlyNQuantification property or class within the SBVR ontology." ;
    rdfs:domain sbvr:ExactlyNQuantificationHasCardinality .

sbvr:ExactlyOneQuantification a owl:Class ;
    rdfs:label "ExactlyOneQuantification" ;
    rdfs:comment "This is the ExactlyOneQuantification property or class within the SBVR ontology." .

sbvr:ExistentialQuantification a owl:Class ;
    rdfs:label "ExistentialQuantification" ;
    rdfs:comment "This is the ExistentialQuantification property or class within the SBVR ontology." .

sbvr:FormalRepresentation a owl:Class ;
    rdfs:label "FormalRepresentation" ;
    rdfs:comment "This is the FormalRepresentation property or class within the SBVR ontology." .

sbvr:GuidanceStatement a rdf:Property,
        owl:Class ;
    rdfs:label "GuidanceStatement" ;
    rdfs:comment "This is the GuidanceStatement property or class within the SBVR ontology." ;
    rdfs:domain sbvr:AuthorityAuthorsGuidanceStatement .

sbvr:Impossibilitystatement a owl:Class ;
    rdfs:label "impossibilityStatement" ;
    rdfs:comment "This is the impossibilityStatement property or class within the SBVR ontology." .

sbvr:Individualverbconcept a owl:Class ;
    rdfs:label "individualVerbConcept" ;
    rdfs:comment "This is the individualVerbConcept property or class within the SBVR ontology." .

sbvr:InFormalRepresentation a owl:Class ;
    rdfs:label "inFormalRepresentation" ;
    rdfs:comment "This is the inFormalRepresentation property or class within the SBVR ontology." .

sbvr:IsFacetOfProposition a owl:Class ;
    rdfs:label "IsFacetOfProposition" ;
    rdfs:comment "This is the IsFacetOfProposition property or class within the SBVR ontology." .

sbvr:IsRoleOfProposition a owl:Class ;
    rdfs:label "IsRoleOfProposition" ;
    rdfs:comment "This is the IsRoleOfProposition property or class within the SBVR ontology." .

sbvr:NecessityStatement a owl:Class ;
    rdfs:label "NecessityStatement" ;
    rdfs:comment "This is the NecessityStatement property or class within the SBVR ontology." .

sbvr:NonNecessityStatement a owl:Class ;
    rdfs:label "NonNecessityStatement" ;
    rdfs:comment "This is the NonNecessityStatement property or class within the SBVR ontology." .

sbvr:NonObligationStatement a owl:Class ;
    rdfs:label "NonObligationStatement" ;
    rdfs:comment "This is the NonObligationStatement property or class within the SBVR ontology." .

sbvr:Note a rdf:Property,
        owl:Class ;
    rdfs:label "Note" ;
    rdfs:comment "This is the note property or class within the SBVR ontology." ;
    rdfs:domain sbvr:NoteCommentsOnMeaning .

sbvr:ObligationStatement a owl:Class ;
    rdfs:label "ObligationStatement" ;
    rdfs:comment "This is the ObligationStatement property or class within the SBVR ontology." .

sbvr:Optionalitystatement a owl:Class ;
    rdfs:label "optionalityStatement" ;
    rdfs:comment "This is the optionalityStatement property or class within the SBVR ontology." .

sbvr:Permissionstatement a owl:Class ;
    rdfs:label "permissionStatement" ;
    rdfs:comment "This is the permissionStatement property or class within the SBVR ontology." .

sbvr:Possibilitystatement a owl:Class ;
    rdfs:label "possibilityStatement" ;
    rdfs:comment "This is the possibilityStatement property or class within the SBVR ontology." .

sbvr:Prohibitionstatement a owl:Class ;
    rdfs:label "prohibitionStatement" ;
    rdfs:comment "This is the prohibitionStatement property or class within the SBVR ontology." .

sbvr:Proposition a rdf:Property,
        owl:Class ;
    rdfs:label "proposition" ;
    rdfs:comment "This is the proposition property or class within the SBVR ontology." ;
    rdfs:domain sbvr:Closedlogicalformulationmeansproposition,
        sbvr:Propositionisbasedonverbconcept,
        sbvr:Statementexpressesproposition .

sbvr:Reference a rdf:Property,
        owl:Class ;
    rdfs:label "Reference" ;
    rdfs:comment "Representation that is the mention or citation of a source of information used to direct a reader elsewhere for additional information about a given concept." ;
    rdfs:domain sbvr:AdoptingAuthorityAdoptsElementOfGuidanceFromOwningAuthorityCitingReference,
        sbvr:ReferencePointsToInformationSource,
        sbvr:ReferenceSupportsMeaning,
        sbvr:SpeechCommunityAdoptsAdoptedDefinitionCitingReference ;
    rdfs:range xsd:anyType .

sbvr:Representation a rdf:Property,
        owl:Class ;
    rdfs:label "representation" ;
    rdfs:comment "This is the representation property or class within the SBVR ontology." ;
    rdfs:domain sbvr:Advice,
        sbvr:AdviceOfContingency,
        sbvr:AdviceOfOptionality,
        sbvr:AdviceOfPermission,
        sbvr:AdviceOfPossibility,
        sbvr:Association,
        sbvr:BehavioralBusinessRule,
        sbvr:Binaryverbconcept,
        sbvr:Businesspolicy,
        sbvr:Businessrule,
        sbvr:Categorization,
        sbvr:Categorizationtype,
        sbvr:Characteristic,
        sbvr:Characteristictype,
        sbvr:Characterization,
        sbvr:Classification,
        sbvr:Communicationcontentiscomposedofrepresentation,
        sbvr:Conceptofthingascomposite,
        sbvr:ConceptOfThingAsContinuant,
        sbvr:ConceptOfThingAsDeveloped,
        sbvr:Conceptofthingasoccurrent,
        sbvr:Conceptofthingasprimitive,
        sbvr:Conceptofthingasunitary,
        sbvr:Conceptofthingexistingdependently,
        sbvr:Conceptofthingexistingindependently,
        sbvr:Concepttype,
        sbvr:Contextualizedconcept,
        sbvr:DefinitionalBusinessRule,
        sbvr:DefinitionalRule,
        sbvr:Derivableconcept,
        sbvr:Elementofgovernance,
        sbvr:Elementofguidance,
        sbvr:Facet,
        sbvr:Fundamentalconcept,
        sbvr:GeneralConcept,
        sbvr:GeneralVerbConcept,
        sbvr:IndividualNounConcept,
        sbvr:Individualverbconcept,
        sbvr:Integer,
        sbvr:IsFacetOfProposition,
        sbvr:IsRoleOfProposition,
        sbvr:LogicalFormulationKind,
        sbvr:NonNegativeInteger,
        sbvr:NounConcept,
        sbvr:Number,
        sbvr:PartitiveVerbConcept,
        sbvr:PositiveInteger,
        sbvr:PropertyAssociation,
        sbvr:Proposition,
        sbvr:Quantity,
        sbvr:Question,
        sbvr:RepresentationHasExpression,
        sbvr:Representationisindesignationcontext,
        sbvr:Representationisinsubjectfield,
        sbvr:Representationrepresentsmeaning,
        sbvr:RepresentationUsesVocabulary,
        sbvr:Role,
        sbvr:Rule,
        sbvr:SituationalRole,
        sbvr:Speechcommunityrepresentationsetincludesrepresentation,
        sbvr:Terminologicaldictionaryincludesrepresentation,
        sbvr:Unitaryverbconcept,
        sbvr:VerbConcept,
        sbvr:VerbConceptRole ;
    rdfs:range xsd:anyType .

sbvr:Restrictedpermissionstatement a owl:Class ;
    rdfs:label "restrictedPermissionStatement" ;
    rdfs:comment "This is the restrictedPermissionStatement property or class within the SBVR ontology." .

sbvr:Restrictedpossibilitystatement a owl:Class ;
    rdfs:label "restrictedPossibilityStatement" ;
    rdfs:comment "This is the restrictedPossibilityStatement property or class within the SBVR ontology." .

sbvr:Rule a owl:Class ;
    rdfs:label "rule" ;
    rdfs:comment "This is the rule property or class within the SBVR ontology." .

sbvr:Fact a owl:Class, sbvr:SententialForm ;
    rdfs:label "Fact" ;
    rdfs:comment "Proposition that is taken as true" .

sbvr:RuleSet a rdf:Property,
        owl:Class ;
    rdfs:label "RuleSet" ;
    rdfs:comment "This is the RuleSet property or class within the SBVR ontology." ;
    rdfs:domain sbvr:BodyOfSharedGuidanceIncludesRuleSet,
        sbvr:RuleSetIncludesElementOfGuidance .

sbvr:Rulestatement a owl:Class ;
    rdfs:label "ruleStatement" ;
    rdfs:comment "This is the ruleStatement property or class within the SBVR ontology." .

sbvr:Speechcommunity a rdf:Property,
        owl:Class ;
    rdfs:label "speechCommunity" ;
    rdfs:comment "This is the speechCommunity property or class within the SBVR ontology." ;
    rdfs:domain sbvr:Expressionisunambiguoustospeechcommunity,
        sbvr:Semanticcommunity,
        sbvr:Semanticcommunityhasspeechcommunity,
        sbvr:SpeechCommunityAdoptsAdoptedDefinitionCitingReference,
        sbvr:Speechcommunitydeterminesspeechcommunityrepresentationset,
        sbvr:Speechcommunityownsowneddefinition,
        sbvr:Speechcommunityownsvocabulary,
        sbvr:Speechcommunityregulatesitsusageofsignifier,
        sbvr:Speechcommunityuseslanguage,
        sbvr:Speechcommunityusesvocabulary,
        sbvr:Vocabularyisdesignedforspeechcommunity ;
    rdfs:range xsd:anyType .

sbvr:Speechcommunityrepresentationset a rdf:Property,
        owl:Class ;
    rdfs:label "speechCommunityRepresentationSet" ;
    rdfs:comment "This is the speechCommunityRepresentationSet property or class within the SBVR ontology." ;
    rdfs:domain sbvr:Speechcommunitydeterminesspeechcommunityrepresentationset,
        sbvr:Speechcommunityrepresentationsetincludesrepresentation .

sbvr:Statement a rdf:Property,
        owl:Class ;
    rdfs:label "statement" ;
    rdfs:comment "This is the statement property or class within the SBVR ontology." ;
    rdfs:domain sbvr:Advice,
        sbvr:AdviceOfContingency,
        sbvr:AdviceOfOptionality,
        sbvr:AdviceOfPermission,
        sbvr:AdviceOfPossibility,
        sbvr:BehavioralBusinessRule,
        sbvr:Businesspolicy,
        sbvr:Businessrule,
        sbvr:Categorization,
        sbvr:Characterization,
        sbvr:Classification,
        sbvr:Closedlogicalformulationformalizesstatement,
        sbvr:DefinitionalBusinessRule,
        sbvr:DefinitionalRule,
        sbvr:Elementofgovernance,
        sbvr:Elementofguidance,
        sbvr:Individualverbconcept,
        sbvr:IsFacetOfProposition,
        sbvr:IsRoleOfProposition,
        sbvr:Proposition,
        sbvr:Rule,
        sbvr:Statementexpressesproposition ;
    rdfs:range xsd:anyType .

sbvr:StatementOfAdviceOfPermission a owl:Class ;
    rdfs:label "StatementOfAdviceOfPermission" ;
    rdfs:comment "This is the StatementOfAdviceOfPermission property or class within the SBVR ontology." .

sbvr:StatementofAdviceOfPossibility a owl:Class ;
    rdfs:label "StatementofAdviceOfPossibility" ;
    rdfs:comment "This is the StatementofAdviceOfPossibility property or class within the SBVR ontology." .

sbvr:Vocabulary a rdf:Property,
        owl:Class ;
    rdfs:label "vocabulary" ;
    rdfs:comment "This is the vocabulary property or class within the SBVR ontology." ;
    rdfs:domain sbvr:RepresentationUsesVocabulary,
        sbvr:Speechcommunityownsvocabulary,
        sbvr:Speechcommunityusesvocabulary,
        sbvr:Terminologicaldictionarypresentsvocabulary,
        sbvr:Vocabularyisdesignedforspeechcommunity,
        sbvr:vocabularyIsExpressedInLanguage,
        sbvr:Vocabularyisusedtoexpressbodyofsharedmeanings,
        sbvr:vocabularyNamespaceIsDerivedFromVocabulary .

sbvr:AdoptedDefinition a rdf:Property,
        owl:Class ;
    rdfs:label "adoptedDefinition" ;
    rdfs:comment "This is the adoptedDefinition property or class within the SBVR ontology." ;
    rdfs:domain sbvr:SpeechCommunityAdoptsAdoptedDefinitionCitingReference ;
    rdfs:range xsd:anyType .

sbvr:Advice a rdf:Property,
        owl:Class ;
    rdfs:label "advice" ;
    rdfs:comment "This is the advice property or class within the SBVR ontology." ;
    rdfs:domain sbvr:AdviceIsDerivedFromBusinessPolicy .

sbvr:AdviceOfContingency a owl:Class ;
    rdfs:label "AdviceOfContingency" ;
    rdfs:comment "This is the AdviceOfContingency property or class within the SBVR ontology." .

sbvr:AdviceOfOptionality a owl:Class ;
    rdfs:label "AdviceOfOptionality" ;
    rdfs:comment "This is the AdviceOfOptionality property or class within the SBVR ontology." .

sbvr:AdviceOfPermission a owl:Class ;
    rdfs:label "AdviceOfPermission" ;
    rdfs:comment "This is the AdviceOfPermission property or class within the SBVR ontology." .

sbvr:AdviceOfPossibility a owl:Class ;
    rdfs:label "AdviceOfPossibility" ;
    rdfs:comment "This is the AdviceOfPossibility property or class within the SBVR ontology." .

sbvr:BagProjection a owl:Class ;
    rdfs:label "BagProjection" ;
    rdfs:comment "This is the bagProjection property or class within the SBVR ontology." .

sbvr:BusinessRule a rdf:Property,
        owl:Class ;
    rdfs:label "BusinessRule" ;
    rdfs:comment "This is the businessRule property or class within the SBVR ontology." ;
    rdfs:domain sbvr:Businessruleisderivedfrombusinesspolicy .

sbvr:ClosedProjection a rdf:Property,
        owl:Class ;
    rdfs:label "ClosedProjection" ;
    rdfs:comment "This is the closedProjection property or class within the SBVR ontology." ;
    rdfs:domain sbvr:ClosedprojectiondefinesNounConcept,
        sbvr:Closedprojectiondefinesverbconcept,
        sbvr:Closedprojectionformalizesdefinition,
        sbvr:Closedprojectionmeansquestion .

sbvr:Conjunction a owl:Class ;
    rdfs:label "Conjunction" ;
    rdfs:comment "This is the conjunction property or class within the SBVR ontology." .

sbvr:DefiniteDescription a owl:Class ;
    rdfs:label "DefiniteDescription" ;
    rdfs:comment "Intensional definition of an individual." .

sbvr:Definition a rdf:Property,
        owl:Class ;
    rdfs:label "Definition" ;
    rdfs:comment "Representation of a concept by a descriptive statement [expression] which serves to differentiate it from related concepts. Representation (as through a word or phrase) expressing the essential nature of a person or thing or class of persons or of things : an answer to the question “what is x?” or “what is an x?”" ;
    rdfs:domain sbvr:Association,
        sbvr:Binaryverbconcept,
        sbvr:Categorizationtype,
        sbvr:Characteristic,
        sbvr:Characteristictype,
        sbvr:Closedprojectionformalizesdefinition,
        sbvr:ConceptHasDefinition,
        sbvr:Conceptofthingascomposite,
        sbvr:ConceptOfThingAsContinuant,
        sbvr:ConceptOfThingAsDeveloped,
        sbvr:Conceptofthingasoccurrent,
        sbvr:Conceptofthingasprimitive,
        sbvr:Conceptofthingasunitary,
        sbvr:Conceptofthingexistingdependently,
        sbvr:Conceptofthingexistingindependently,
        sbvr:Concepttype,
        sbvr:Contextualizedconcept,
        sbvr:Derivableconcept,
        sbvr:Facet,
        sbvr:Fundamentalconcept,
        sbvr:GeneralConcept,
        sbvr:GeneralVerbConcept,
        sbvr:IndividualNounConcept,
        sbvr:Integer,
        sbvr:LogicalFormulationKind,
        sbvr:NonNegativeInteger,
        sbvr:NounConcept,
        sbvr:Number,
        sbvr:PartitiveVerbConcept,
        sbvr:PositiveInteger,
        sbvr:PropertyAssociation,
        sbvr:Quantity,
        sbvr:Role,
        sbvr:SituationalRole,
        sbvr:Unitaryverbconcept,
        sbvr:VerbConcept,
        sbvr:VerbConceptRole ;
    rdfs:range xsd:anyType .

sbvr:Disjunction a owl:Class ;
    rdfs:label "disjunction" ;
    rdfs:comment "This is the disjunction property or class within the SBVR ontology." .

sbvr:Elementofguidance a rdf:Property,
        owl:Class ;
    rdfs:label "elementOfGuidance" ;
    rdfs:comment "This is the elementOfGuidance property or class within the SBVR ontology." ;
    rdfs:domain sbvr:AdoptingAuthorityAdoptsElementOfGuidanceFromOwningAuthorityCitingReference,
        sbvr:AuthorityDefinesElementofGuidance,
        sbvr:Bodyofsharedguidanceincludeselementofguidance,
        sbvr:Elementofguidanceacknowledgesaspossiblestateofaffairs,
        sbvr:Elementofguidanceisinthejurisdictionofauthority,
        sbvr:Elementofguidancenecessitatesstateofaffairs,
        sbvr:Elementofguidancepermitsstateofaffairs,
        sbvr:RuleSetIncludesElementOfGuidance ;
    rdfs:range xsd:anyType .

sbvr:Equivalence a owl:Class ;
    rdfs:label "equivalence" ;
    rdfs:comment "This is the equivalence property or class within the SBVR ontology." .

sbvr:Exclusivedisjunction a owl:Class ;
    rdfs:label "exclusiveDisjunction" ;
    rdfs:comment "This is the exclusiveDisjunction property or class within the SBVR ontology." .

sbvr:Extensionaldefinition a owl:Class ;
    rdfs:label "extensionalDefinition" ;
    rdfs:comment "This is the extensionalDefinition property or class within the SBVR ontology." .

sbvr:IntensionalDefinition a rdf:Property,
        owl:Class ;
    rdfs:label "IntensionalDefinition" ;
    rdfs:comment "This is the IntensionalDefinition property or class within the SBVR ontology." ;
    rdfs:domain sbvr:IntensionalDefinitionusesdelimitingcharacteristic .

sbvr:Nandformulation a owl:Class ;
    rdfs:label "nandFormulation" ;
    rdfs:comment "This is the nandFormulation property or class within the SBVR ontology." .

sbvr:Norformulation a owl:Class ;
    rdfs:label "norFormulation" ;
    rdfs:comment "This is the norFormulation property or class within the SBVR ontology." .

sbvr:Nounform a owl:Class ;
    rdfs:label "nounForm" ;
    rdfs:comment "This is the nounForm property or class within the SBVR ontology." .

sbvr:NumericrangeQuantification a rdf:Property,
        owl:Class ;
    rdfs:label "numericRangeQuantification" ;
    rdfs:comment "This is the numericRangeQuantification property or class within the SBVR ontology." ;
    rdfs:domain sbvr:NumericrangeQuantificationhasmaximumcardinality,
        sbvr:NumericrangeQuantificationhasminimumcardinality .

sbvr:Owneddefinition a rdf:Property,
        owl:Class ;
    rdfs:label "ownedDefinition" ;
    rdfs:comment "This is the ownedDefinition property or class within the SBVR ontology." ;
    rdfs:domain sbvr:Speechcommunityownsowneddefinition .

sbvr:Projection a rdf:Property,
        owl:Class ;
    rdfs:label "projection" ;
    rdfs:comment "This is the projection property or class within the SBVR ontology." ;
    rdfs:domain sbvr:Aggregationformulation,
        sbvr:Answernominalization,
        sbvr:Logicalformulationconstrainsprojection,
        sbvr:NounConceptnominalization,
        sbvr:Projectingformulationhasprojection,
        sbvr:Projectionhasauxiliaryvariable,
        sbvr:Projectionisonvariable,
        sbvr:QuestionNominalization,
        sbvr:VerbConceptnominalization ;
    rdfs:range xsd:anyType .

sbvr:ReferenceScheme a rdf:Property,
        owl:Class ;
    rdfs:label "ReferenceScheme" ;
    rdfs:comment "This is the ReferenceScheme property or class within the SBVR ontology." ;
    rdfs:domain sbvr:Association,
        sbvr:Binaryverbconcept,
        sbvr:Categorizationtype,
        sbvr:Characteristic,
        sbvr:Characteristictype,
        sbvr:Conceptofthingascomposite,
        sbvr:ConceptOfThingAsContinuant,
        sbvr:ConceptOfThingAsDeveloped,
        sbvr:Conceptofthingasoccurrent,
        sbvr:Conceptofthingasprimitive,
        sbvr:Conceptofthingasunitary,
        sbvr:Conceptofthingexistingdependently,
        sbvr:Conceptofthingexistingindependently,
        sbvr:Concepttype,
        sbvr:Contextualizedconcept,
        sbvr:Derivableconcept,
        sbvr:Facet,
        sbvr:Fundamentalconcept,
        sbvr:GeneralConcept,
        sbvr:GeneralVerbConcept,
        sbvr:IndividualNounConcept,
        sbvr:Integer,
        sbvr:LogicalFormulationKind,
        sbvr:NonNegativeInteger,
        sbvr:NounConcept,
        sbvr:Number,
        sbvr:PartitiveVerbConcept,
        sbvr:PositiveInteger,
        sbvr:PropertyAssociation,
        sbvr:Quantity,
        sbvr:ReferenceSchemeextensionallyusesverbconceptrole,
        sbvr:ReferenceSchemeisforconcept,
        sbvr:ReferenceSchemesimplyusesverbconceptrole,
        sbvr:ReferenceSchemeUsesCharacteristic,
        sbvr:Role,
        sbvr:SituationalRole,
        sbvr:Unitaryverbconcept,
        sbvr:VerbConcept,
        sbvr:VerbConceptRole ;
    rdfs:range xsd:anyType .

sbvr:Semanticcommunity a rdf:Property,
        owl:Class ;
    rdfs:label "semanticCommunity" ;
    rdfs:comment "This is the semanticCommunity property or class within the SBVR ontology." ;
    rdfs:domain sbvr:Bodyofsharedmeaningsunitessemanticcommunity,
        sbvr:Semanticcommunityhasspeechcommunity,
        sbvr:Semanticcommunitysharesunderstandingofconcept .

sbvr:SententialForm a owl:Class ;
    rdfs:label "SententialForm" ;
    rdfs:comment "Verb concept wording that is a pattern or template that can be used for stating a proposition based on a verb concept." .

sbvr:SetProjection a owl:Class ;
    rdfs:label "SetProjection" ;
    rdfs:comment "This is the SetProjection property or class within the SBVR ontology." .

sbvr:SpeechCommunityAdoptsAdoptedDefinitionCitingReference a owl:Class ;
    rdfs:label "SpeechCommunityAdoptsAdoptedDefinitionCitingReference" ;
    rdfs:comment "The speech community agrees that the definition identified by the reference can serve as the adopted definition" .

sbvr:VerbConceptwording a rdf:Property,
        owl:Class ;
    rdfs:label "verbConceptWording" ;
    rdfs:comment "This is the verbConceptWording property or class within the SBVR ontology." ;
    rdfs:domain sbvr:Association,
        sbvr:Binaryverbconcept,
        sbvr:Characteristic,
        sbvr:GeneralVerbConcept,
        sbvr:PartitiveVerbConcept,
        sbvr:Placeholderisinverbconceptwording,
        sbvr:PropertyAssociation,
        sbvr:Unitaryverbconcept,
        sbvr:VerbConcept,
        sbvr:VerbConcepthasverbconceptwording,
        sbvr:VerbConceptWordinginCorporatesVerbSymbol,
        sbvr:VerbConceptWordingIsInNamespace ;
    rdfs:range xsd:anyType .

sbvr:AdoptingAuthorityAdoptsElementOfGuidanceFromOwningAuthorityCitingReference a owl:Class ;
    rdfs:label "AdoptingAuthorityAdoptsElementOfGuidanceFromOwningAuthorityCitingReference" ;
    rdfs:comment "This is the AdoptingAuthorityAdoptsElementOfGuidanceFromOwningAuthorityCitingReference property or class within the SBVR ontology." .

sbvr:Auxiliaryvariable a rdf:Property,
        owl:Class ;
    rdfs:label "auxiliaryVariable" ;
    rdfs:comment "This is the auxiliaryVariable property or class within the SBVR ontology." ;
    rdfs:domain sbvr:Bagprojection,
        sbvr:Closedprojection,
        sbvr:Projection,
        sbvr:Projectionhasauxiliaryvariable,
        sbvr:SetProjection ;
    rdfs:range xsd:anyType .

sbvr:Businesspolicy a rdf:Property,
        owl:Class ;
    rdfs:label "businessPolicy" ;
    rdfs:comment "This is the businessPolicy property or class within the SBVR ontology." ;
    rdfs:domain sbvr:AdviceIsDerivedFromBusinessPolicy,
        sbvr:Businessruleisderivedfrombusinesspolicy .

sbvr:Designation a rdf:Property,
        owl:Class ;
    rdfs:label "designation" ;
    rdfs:comment "Representation of a concept by a sign which denotes it",
        "This is the designation property or class within the SBVR ontology." ;
    rdfs:domain sbvr:Association,
        sbvr:Binaryverbconcept,
        sbvr:Categorizationtype,
        sbvr:Characteristic,
        sbvr:Characteristictype,
        sbvr:ConceptHasDesignation,
        sbvr:Conceptofthingascomposite,
        sbvr:ConceptOfThingAsContinuant,
        sbvr:ConceptOfThingAsDeveloped,
        sbvr:Conceptofthingasoccurrent,
        sbvr:Conceptofthingasprimitive,
        sbvr:Conceptofthingasunitary,
        sbvr:Conceptofthingexistingdependently,
        sbvr:Conceptofthingexistingindependently,
        sbvr:Concepttype,
        sbvr:Contextualizedconcept,
        sbvr:Derivableconcept,
        sbvr:DesignationHasSignifier,
        sbvr:designationIsInNamespace,
        sbvr:Facet,
        sbvr:Fundamentalconcept,
        sbvr:GeneralConcept,
        sbvr:GeneralVerbConcept,
        sbvr:IndividualNounConcept,
        sbvr:Integer,
        sbvr:LogicalFormulationKind,
        sbvr:NonNegativeInteger,
        sbvr:NounConcept,
        sbvr:Number,
        sbvr:PartitiveVerbConcept,
        sbvr:Placeholderusesdesignation,
        sbvr:PositiveInteger,
        sbvr:PropertyAssociation,
        sbvr:Quantity,
        sbvr:Role,
        sbvr:SituationalRole,
        sbvr:Unitaryverbconcept,
        sbvr:VerbConcept,
        sbvr:VerbConceptRole ;
    rdfs:range xsd:anyType .

sbvr:Elementofgovernance a owl:Class ;
    rdfs:label "elementOfGovernance" ;
    rdfs:comment "This is the elementOfGovernance property or class within the SBVR ontology." .

sbvr:Icon a owl:Class ;
    rdfs:label "icon" ;
    rdfs:comment "This is the icon property or class within the SBVR ontology." .

sbvr:Name a rdf:Property,
        owl:Class ;
    rdfs:label "Name" ;
    rdfs:comment "This is the name property or class within the SBVR ontology.",
        "Verbal designation of an individual noun concept." ;
    rdfs:domain sbvr:AdoptedDefinition,
        sbvr:AdoptingAuthorityAdoptsElementOfGuidanceFromOwningAuthorityCitingReference,
        sbvr:Advice,
        sbvr:AdviceOfContingency,
        sbvr:AdviceOfOptionality,
        sbvr:AdviceOfPermission,
        sbvr:AdviceOfPossibility,
        sbvr:Advicestatement,
        sbvr:Aggregationformulation,
        sbvr:Answernominalization,
        sbvr:Association,
        sbvr:AtLeastNQuantification,
        sbvr:AtMostNQuantification,
        sbvr:AtMostOneQuantification,
        sbvr:Atomicformulation,
        sbvr:Attributivenamespace,
        sbvr:Authority,
        sbvr:Auxiliaryvariable,
        sbvr:Bagprojection,
        sbvr:BehavioralBusinessRule,
        sbvr:BehavioralBusinessRulestatement,
        sbvr:Binaryverbconcept,
        sbvr:Bodyofsharedconcepts,
        sbvr:Bodyofsharedguidance,
        sbvr:Bodyofsharedmeanings,
        sbvr:Businesspolicy,
        sbvr:Businesspolicystatement,
        sbvr:Businessrule,
        sbvr:Businessvocabulary,
        sbvr:Categorization,
        sbvr:Categorizationscheme,
        sbvr:Categorizationtype,
        sbvr:Characteristic,
        sbvr:Characteristictype,
        sbvr:Characterization,
        sbvr:Classification,
        sbvr:Closedlogicalformulation,
        sbvr:Closedprojection,
        sbvr:Communicationcontent,
        sbvr:Conceptofthingascomposite,
        sbvr:ConceptOfThingAsContinuant,
        sbvr:ConceptOfThingAsDeveloped,
        sbvr:Conceptofthingasoccurrent,
        sbvr:Conceptofthingasprimitive,
        sbvr:Conceptofthingasunitary,
        sbvr:Conceptofthingexistingdependently,
        sbvr:Conceptofthingexistingindependently,
        sbvr:Concepttype,
        sbvr:Conjunction,
        sbvr:Contextualizedconcept,
        sbvr:Contingencystatement,
        sbvr:Definitedescription,
        sbvr:Definition,
        sbvr:DefinitionalBusinessRule,
        sbvr:DefinitionalRule,
        sbvr:DefinitionalRuleStatement,
        sbvr:Derivableconcept,
        sbvr:Description,
        sbvr:Descriptiveexample,
        sbvr:Designation,
        sbvr:Disjunction,
        sbvr:Elementofgovernance,
        sbvr:Elementofguidance,
        sbvr:ElementsOfConceptSystemStructure,
        sbvr:Enforcementlevel,
        sbvr:Equivalence,
        sbvr:ExactlyNQuantification,
        sbvr:ExactlyOneQuantification,
        sbvr:Exclusivedisjunction,
        sbvr:ExistentialQuantification,
        sbvr:Extensionaldefinition,
        sbvr:Facet,
        sbvr:FormalRepresentation,
        sbvr:Fundamentalconcept,
        sbvr:GeneralConcept,
        sbvr:GeneralVerbConcept,
        sbvr:GuidanceStatement,
        sbvr:Icon,
        sbvr:Implication,
        sbvr:Impossibilitystatement,
        sbvr:IndividualNounConcept,
        sbvr:Individualverbconcept,
        sbvr:InFormalRepresentation,
        sbvr:Instantiationformulation,
        sbvr:Integer,
        sbvr:IntensionalDefinition,
        sbvr:IsFacetOfProposition,
        sbvr:IsRoleOfProposition,
        sbvr:Language,
        sbvr:LogicalFormulationKind,
        sbvr:Logicalnegation,
        sbvr:Name,
        sbvr:Namespace,
        sbvr:Nandformulation,
        sbvr:Necessityformulation,
        sbvr:NecessityStatement,
        sbvr:NonNecessityStatement,
        sbvr:NonObligationStatement,
        sbvr:NonNegativeInteger,
        sbvr:Nonverbaldesignation,
        sbvr:Norformulation,
        sbvr:Note,
        sbvr:NounConcept,
        sbvr:NounConceptnominalization,
        sbvr:Nounform,
        sbvr:Number,
        sbvr:NumericrangeQuantification,
        sbvr:Objectification,
        sbvr:Obligationformulation,
        sbvr:ObligationStatement,
        sbvr:Optionalitystatement,
        sbvr:Owneddefinition,
        sbvr:PartitiveVerbConcept,
        sbvr:Permissibilityformulation,
        sbvr:Permissionstatement,
        sbvr:Placeholder,
        sbvr:PositiveInteger,
        sbvr:Possibilityformulation,
        sbvr:Possibilitystatement,
        sbvr:Preferreddesignation,
        sbvr:Prohibiteddesignation,
        sbvr:Prohibitionstatement,
        sbvr:Projection,
        sbvr:Property,
        sbvr:PropertyAssociation,
        sbvr:Proposition,
        sbvr:Propositionnominalization,
        sbvr:Quantity,
        sbvr:Question,
        sbvr:QuestionNominalization,
        sbvr:Reference,
        sbvr:ReferenceScheme,
        sbvr:Representation,
        sbvr:RepresentationFormality,
        sbvr:Restrictedpermissionstatement,
        sbvr:Restrictedpossibilitystatement,
        sbvr:Role,
        sbvr:Rolebinding,
        sbvr:Rule,
        sbvr:Rulebook,
        sbvr:RuleSet,
        sbvr:Rulestatement,
        sbvr:SbvrRulebook,
        sbvr:Segmentation,
        sbvr:Semanticcommunity,
        sbvr:SententialForm,
        sbvr:SetProjection,
        sbvr:SituationalRole,
        sbvr:Speechcommunity,
        sbvr:SpeechCommunityAdoptsAdoptedDefinitionCitingReference,
        sbvr:Speechcommunityrepresentationset,
        sbvr:Statement,
        sbvr:StatementOfAdviceOfPermission,
        sbvr:StatementofAdviceOfPossibility,
        sbvr:Stateofaffairs,
        sbvr:Subjectfield,
        sbvr:Term,
        sbvr:Terminologicaldictionary,
        sbvr:Text,
        sbvr:URI,
        sbvr:Unitaryverbconcept,
        sbvr:UniversalQuantification,
        sbvr:Variable,
        sbvr:VerbConcept,
        sbvr:VerbConceptnominalization,
        sbvr:VerbConceptRole,
        sbvr:VerbConceptRoledesignation,
        sbvr:VerbConceptwording,
        sbvr:Verbsymbol,
        sbvr:Viewpoint,
        sbvr:Vocabulary,
        sbvr:VocabularyNamespace,
        sbvr:WhetherOrNotFormulation ;
    rdfs:range xsd:anyType .

sbvr:Nonverbaldesignation a owl:Class ;
    rdfs:label "nonverbalDesignation" ;
    rdfs:comment "This is the nonverbalDesignation property or class within the SBVR ontology." .

sbvr:Preferreddesignation a owl:Class ;
    rdfs:label "preferredDesignation" ;
    rdfs:comment "This is the preferredDesignation property or class within the SBVR ontology." .

sbvr:Prohibiteddesignation a owl:Class ;
    rdfs:label "prohibitedDesignation" ;
    rdfs:comment "This is the prohibitedDesignation property or class within the SBVR ontology." .

sbvr:Variable a rdf:Property,
        owl:Class ;
    rdfs:label "variable" ;
    rdfs:comment "This is the variable property or class within the SBVR ontology." ;
    rdfs:domain sbvr:Logicalformulationrestrictsvariable,
        sbvr:Projectionisonvariable,
        sbvr:QuantificationIntroducesVariable,
        sbvr:Variablehasprojectionposition,
        sbvr:Variableisfreewithinsemanticformulation,
        sbvr:Variablemapstoverbconceptrole,
        sbvr:Variablerangesoverconcept .

sbvr:VerbConceptRoledesignation a owl:Class ;
    rdfs:label "verbConceptRoleDesignation" ;
    rdfs:comment "This is the verbConceptRoleDesignation property or class within the SBVR ontology." .

sbvr:Verbsymbol a rdf:Property,
        owl:Class ;
    rdfs:label "verbSymbol" ;
    rdfs:comment "This is the verbSymbol property or class within the SBVR ontology." ;
    rdfs:domain sbvr:VerbConceptWordinginCorporatesVerbSymbol .

sbvr:Implication a rdf:Property,
        owl:Class ;
    rdfs:label "implication" ;
    rdfs:comment "This is the implication property or class within the SBVR ontology." ;
    rdfs:domain sbvr:Implicationhasantecedent,
        sbvr:Implicationhasconsequent .

sbvr:Placeholder a rdf:Property,
        owl:Class ;
    rdfs:label "placeholder" ;
    rdfs:comment "This is the placeholder property or class within the SBVR ontology." ;
    rdfs:domain sbvr:Nounform,
        sbvr:Placeholderisatstartingcharacterposition,
        sbvr:Placeholderisinverbconceptwording,
        sbvr:Placeholderusesdesignation,
        sbvr:SententialForm,
        sbvr:VerbConceptwording ;
    rdfs:range xsd:anyType .

sbvr:WhetherOrNotFormulation a rdf:Property,
        owl:Class ;
    rdfs:label "WhetherOrNotFormulation" ;
    rdfs:comment "This is the WhetherOrNotFormulation property or class within the SBVR ontology." ;
    rdfs:domain sbvr:WhetherOrNotFormulationHasConsequent,
        sbvr:WhetherOrNotFormulationHasInconsequent .

sbvr:BehavioralBusinessRule a rdf:Property,
        owl:Class ;
    rdfs:label "BehavioralBusinessRule" ;
    rdfs:comment "This is the BehavioralBusinessRule property or class within the SBVR ontology." ;
    rdfs:domain sbvr:BehavioralBusinessRuleHasEnforcementLevel .

sbvr:Term a owl:Class ;
    rdfs:label "Term" ;
    rdfs:comment "A verbal designation of a general concept that is in a given subject field" ;
    rdfs:subClassOf skos:Concept .

sbvr:Conceptofthingascomposite a owl:Class ;
    rdfs:label "conceptOfThingAsComposite" ;
    rdfs:comment "This is the conceptOfThingAsComposite property or class within the SBVR ontology." .

sbvr:ConceptOfThingAsContinuant a owl:Class ;
    rdfs:label "ConceptOfThingAsContinuant" ;
    rdfs:comment "This is the ConceptOfThingAsContinuant property or class within the SBVR ontology." .

sbvr:ConceptOfThingAsDeveloped a owl:Class ;
    rdfs:label "ConceptOfThingAsDeveloped" ;
    rdfs:comment "This is the ConceptOfThingAsDeveloped property or class within the SBVR ontology." .

sbvr:Conceptofthingasoccurrent a owl:Class ;
    rdfs:label "conceptOfThingAsOccurrent" ;
    rdfs:comment "This is the conceptOfThingAsOccurrent property or class within the SBVR ontology." .

sbvr:Conceptofthingasprimitive a owl:Class ;
    rdfs:label "conceptOfThingAsPrimitive" ;
    rdfs:comment "This is the conceptOfThingAsPrimitive property or class within the SBVR ontology." .

sbvr:Conceptofthingasunitary a owl:Class ;
    rdfs:label "conceptOfThingAsUnitary" ;
    rdfs:comment "This is the conceptOfThingAsUnitary property or class within the SBVR ontology." .

sbvr:Conceptofthingexistingdependently a owl:Class ;
    rdfs:label "conceptOfThingExistingDependently" ;
    rdfs:comment "This is the conceptOfThingExistingDependently property or class within the SBVR ontology." .

sbvr:Conceptofthingexistingindependently a owl:Class ;
    rdfs:label "conceptOfThingExistingIndependently" ;
    rdfs:comment "This is the conceptOfThingExistingIndependently property or class within the SBVR ontology." .

sbvr:Contextualizedconcept a owl:Class ;
    rdfs:label "contextualizedConcept" ;
    rdfs:comment "This is the contextualizedConcept property or class within the SBVR ontology." .

sbvr:Derivableconcept a owl:Class ;
    rdfs:label "derivableConcept" ;
    rdfs:comment "This is the derivableConcept property or class within the SBVR ontology." .

sbvr:Facet a rdf:Property,
        owl:Class ;
    rdfs:label "facet" ;
    rdfs:comment "This is the facet property or class within the SBVR ontology." ;
    rdfs:domain sbvr:Association,
        sbvr:Binaryverbconcept,
        sbvr:Categorizationtype,
        sbvr:Characteristic,
        sbvr:Characteristictype,
        sbvr:ConceptHasFacet,
        sbvr:Conceptofthingascomposite,
        sbvr:ConceptOfThingAsContinuant,
        sbvr:ConceptOfThingAsDeveloped,
        sbvr:Conceptofthingasoccurrent,
        sbvr:Conceptofthingasprimitive,
        sbvr:Conceptofthingasunitary,
        sbvr:Conceptofthingexistingdependently,
        sbvr:Conceptofthingexistingindependently,
        sbvr:Concepttype,
        sbvr:Contextualizedconcept,
        sbvr:Derivableconcept,
        sbvr:Facet,
        sbvr:Fundamentalconcept,
        sbvr:GeneralConcept,
        sbvr:GeneralVerbConcept,
        sbvr:IndividualNounConcept,
        sbvr:Integer,
        sbvr:LogicalFormulationKind,
        sbvr:NonNegativeInteger,
        sbvr:NounConcept,
        sbvr:Number,
        sbvr:PartitiveVerbConcept,
        sbvr:PositiveInteger,
        sbvr:PropertyAssociation,
        sbvr:Quantity,
        sbvr:Role,
        sbvr:SituationalRole,
        sbvr:Unitaryverbconcept,
        sbvr:VerbConcept,
        sbvr:VerbConceptRole ;
    rdfs:range xsd:anyType .

sbvr:IndividualNounConcept a owl:Class ;
    rdfs:label "IndividualNounConcept" ;
    rdfs:comment "Noun concept that corresponds to at most one thing in all possible worlds." .

sbvr:NounConcept a rdf:Property,
        owl:Class ;
    rdfs:label "NounConcept" ;
    rdfs:comment "This is the NounConcept property or class within the SBVR ontology." ;
    rdfs:domain sbvr:ClosedprojectiondefinesNounConcept .

sbvr:Number a owl:Class ;
    rdfs:label "Number" ;
    rdfs:comment "This is the number property or class within the SBVR ontology." .

sbvr:Quantity a owl:Class ;
    rdfs:label "quantity" ;
    rdfs:comment "This is the quantity property or class within the SBVR ontology." .

sbvr:Role a rdf:Property,
        owl:Class ;
    rdfs:label "role" ;
    rdfs:comment "This is the role property or class within the SBVR ontology." ;
    rdfs:domain sbvr:RoleRangesOverGeneralConcept .

sbvr:Integer a owl:Class ;
    rdfs:label "integer" ;
    rdfs:comment "This is the integer property or class within the SBVR ontology." .

sbvr:NonNegativeInteger a owl:Class ;
    rdfs:label "nonnegativeInteger" ;
    rdfs:comment "This is the nonnegativeInteger property or class within the SBVR ontology." .

sbvr:PositiveInteger a owl:Class ;
    rdfs:label "positiveInteger" ;
    rdfs:comment "This is the positiveInteger property or class within the SBVR ontology." .

sbvr:VerbConceptRole a rdf:Property,
        owl:Class ;
    rdfs:label "verbConceptRole" ;
    rdfs:comment "This is the verbConceptRole property or class within the SBVR ontology." ;
    rdfs:domain sbvr:Association,
        sbvr:Binaryverbconcept,
        sbvr:Characteristic,
        sbvr:GeneralVerbConcept,
        sbvr:PartitiveVerbConcept,
        sbvr:PropertyAssociation,
        sbvr:ReferenceSchemeextensionallyusesverbconceptrole,
        sbvr:ReferenceSchemesimplyusesverbconceptrole,
        sbvr:Unitaryverbconcept,
        sbvr:Variablemapstoverbconceptrole,
        sbvr:VerbConcept,
        sbvr:VerbConceptRoleHasRolebinding,
        sbvr:VerbConceptRoleIsInVerbConcept ;
    rdfs:range xsd:anyType .

sbvr:Association a owl:Class ;
    rdfs:label "association" ;
    rdfs:comment "This is the association property or class within the SBVR ontology." .

sbvr:Binaryverbconcept a owl:Class ;
    rdfs:label "binaryVerbConcept" ;
    rdfs:comment "This is the binaryVerbConcept property or class within the SBVR ontology." .

sbvr:Categorizationtype a rdf:Property,
        owl:Class ;
    rdfs:label "categorizationType" ;
    rdfs:comment "This is the categorizationType property or class within the SBVR ontology." ;
    rdfs:domain sbvr:Categorizationtype,
        sbvr:Categorizationtypeisforgeneralconcept,
        sbvr:Characteristictype,
        sbvr:Concepttype,
        sbvr:Fundamentalconcept,
        sbvr:GeneralConcept,
        sbvr:LogicalFormulationKind,
        sbvr:SituationalRole ;
    rdfs:range xsd:anyType .

sbvr:Characteristic a rdf:Property,
        owl:Class ;
    rdfs:label "characteristic" ;
    rdfs:comment "This is the characteristic property or class within the SBVR ontology." ;
    rdfs:domain sbvr:ConceptIncorporatesCharacteristic,
        sbvr:ReferenceSchemeUsesCharacteristic .

sbvr:CharacteristicType a owl:Class ;
    rdfs:label "CharacteristicType" ;
    rdfs:comment "This is the characteristicType property or class within the SBVR ontology." .

sbvr:ConceptType a owl:Class ;
    rdfs:label "ConceptType" ;
    rdfs:comment "This is the conceptType property or class within the SBVR ontology." .

sbvr:FundamentalConcept a owl:Class ;
    rdfs:label "FundamentalConcept" ;
    rdfs:comment "General concept whose real-world individuals are perceived by a given semantic community as being in their essence, apart from any situation in which they are involved or viewpoint from which they are considered" .

sbvr:GeneralConcept a rdf:Property,
        owl:Class ;
    rdfs:label "generalConcept" ;
    rdfs:comment "This is the generalConcept property or class within the SBVR ontology." ;
    rdfs:domain sbvr:Categorizationschemeisforgeneralconcept,
        sbvr:Categorizationtypeisforgeneralconcept,
        sbvr:GeneralConceptobjectifiesverbconcept,
        sbvr:RoleRangesOverGeneralConcept .

sbvr:GeneralVerbConcept a owl:Class ;
    rdfs:label "generalVerbConcept" ;
    rdfs:comment "This is the generalVerbConcept property or class within the SBVR ontology." .

sbvr:LogicalFormulationKind a owl:Class ;
    rdfs:label "logicalFormulationKind" ;
    rdfs:comment "This is the logicalFormulationKind property or class within the SBVR ontology." .

sbvr:PartitiveVerbConcept a owl:Class ;
    rdfs:label "partitiveVerbConcept" ;
    rdfs:comment "This is the partitiveVerbConcept property or class within the SBVR ontology." .

sbvr:PropertyAssociation a owl:Class ;
    rdfs:label "propertyAssociation" ;
    rdfs:comment "This is the propertyAssociation property or class within the SBVR ontology." .

sbvr:SituationalRole a owl:Class ;
    rdfs:label "situationalRole" ;
    rdfs:comment "This is the situationalRole property or class within the SBVR ontology." .

sbvr:Unitaryverbconcept a owl:Class ;
    rdfs:label "unitaryVerbConcept" ;
    rdfs:comment "This is the unitaryVerbConcept property or class within the SBVR ontology." .

sbvr:VerbConcept a rdf:Property,
        owl:Class ;
    rdfs:label "verbConcept" ;
    rdfs:comment "This is the verbConcept property or class within the SBVR ontology." ;
    rdfs:domain sbvr:Atomicformulationisbasedonverbconcept,
        sbvr:Closedprojectiondefinesverbconcept,
        sbvr:GeneralConceptobjectifiesverbconcept,
        sbvr:Propositionisbasedonverbconcept,
        sbvr:VerbConcepthasverbconceptwording,
        sbvr:VerbConceptRoleIsInVerbConcept .